Complete proofs for simplicial_complex/map/subcomplex files.

src/simplicial_map.lean
@@ -36,6 +36,28 @@ structure simplicial_map
 := mk :: (map : α → β)
          (is_simplicial : is_simplicial_map X Y map)
 
+lemma simplicial_map_restrict_is_simplicial
+    (X Y : simplicial_complex α)
+    (Z : simplicial_complex β)
+    (f : simplicial_map X Z)
+  : Y ⊆ X → is_simplicial_map Y Z f.map
+:= begin
+  simp only [is_simplicial_map, is_subcomplex],
+  intros Y_sub_X s s_in_Y,
+  simp only [set.subset_def] at Y_sub_X,
+  specialize Y_sub_X s s_in_Y,
+  apply f.is_simplicial,
+  assumption,
+end
+
+def simplicial_map.restrict
+    {X Y : simplicial_complex α}
+    {Z : simplicial_complex β}
+    (f : simplicial_map X Z)
+    (Y_sub_X : Y ⊆ X)
+  : simplicial_map Y Z
+:= simplicial_map.mk f.map (simplicial_map_restrict_is_simplicial X Y Z f Y_sub_X)
+
 def simplicial_map_lift
     {X : simplicial_complex α}
     {Y : simplicial_complex β}
@@ -46,7 +68,6 @@ def simplicial_map_lift
 def simplicial_image
     (X : simplicial_complex α)
     (f : α → β)
-    (f_inj : set.inj_on f (vertices X))
   : simplicial_complex β
 := simplicial_complex.mk
     ({(finset.image f s) | s ∈ X.simplices})
@@ -65,59 +86,118 @@ def simplicial_image
       rw [set.mem_set_of] at *,
       choose u Hu u_img using s_in_img,
 
-      have Hf : set.inj_on f (f⁻¹' ↑t), from
-      begin
-        sorry
-      end,
-      use (finset.preimage t f Hf),
-      split,
+      rw [←u_img, ←finset.coe_subset, finset.coe_image, finset.subset_image_iff] at t_sset_s,
+      choose v v_sset_u v_img using t_sset_s,
 
+      use v, split,
       apply X.subset_closed u,
       assumption,
-      rw [finset.subset_iff] at *,
-      intros x x_in_preimg,
-      rw [finset.mem_preimage] at x_in_preimg,
-      specialize t_sset_s x_in_preimg,
-      rw [finset.ext_iff] at u_img,
-      specialize u_img (f x),
-      cases u_img,
-      specialize u_img_mpr t_sset_s,
-      have Hu : set.inj_on f u, by sorry,
-      sorry,
 
-      rw [finset.ext_iff],
-      intro x,
-      rw [finset.mem_image],
-      split,
-
-      intro y_in_preimg,
-      choose y Hy y_in_preimg using y_in_preimg,
-      rw [finset.mem_preimage, y_in_preimg] at Hy,
+      rw [←finset.coe_subset],
       assumption,
-
-      intro x_in_t,
-      rw [finset.ext_iff] at u_img,
-      specialize u_img x,
-      cases u_img,
-      rw [finset.subset_iff] at t_sset_s,
-      specialize t_sset_s x_in_t,
-      specialize u_img_mpr t_sset_s,
-      rw [finset.mem_image] at u_img_mpr,
-      choose y Hy y_img using u_img_mpr,
-      rw [←y_img, ←finset.mem_preimage] at x_in_t,
-      use y, split; assumption,
+      assumption,
     end)
 
 lemma map_is_simplicial_onto_image
     (X : simplicial_complex α)
     (f : α → β)
-    (f_inj : set.inj_on f (vertices X))
-  : is_simplicial_map X (simplicial_image X f f_inj) f
+  : is_simplicial_map X (simplicial_image X f) f
 := begin
   unfold is_simplicial_map,
   intros s s_in_X,
   simp only[simplicial_image, set.mem_set_of],
   use s, split; tauto,
+end
+
+def simplicial_map.onto_image
+    {X : simplicial_complex α}
+    {Z : simplicial_complex β}
+    (f : simplicial_map X Z)
+  : simplicial_map X (simplicial_image X f.map)
+:= simplicial_map.mk f.map (map_is_simplicial_onto_image X f.map)
+
+lemma simplicial_image_vertices
+    (X : simplicial_complex α)
+    (f : α → β)
+  : vertices (simplicial_image X f) = f '' (vertices X)
+:= begin
+  simp only [vertices_set_of, simplicial_image, set.image, set.ext_iff, set.mem_set_of],
+  intro y,
+  split,
+
+  intro y_in_vert_img,
+  choose t t_in_img y_in_t using y_in_vert_img,
+  choose s s_in_X fs_eq_t using t_in_img,
+  rw [←fs_eq_t, finset.mem_image] at y_in_t,
+  choose x x_in_s fx_eq_y using y_in_t,
+  use x, split,
+  use s, split; assumption,
+  assumption,
+
+  intro y_in_img_vert,
+  choose x x_in_X fx_eq_y using y_in_img_vert,
+  choose s s_in_X x_in_s using x_in_X,
+  use (finset.image f s), split,
+  use s, split,
+  assumption,
+  refl,
+  rw [←fx_eq_y],
+  apply finset.mem_image_of_mem,
+  assumption,
+end
+
+notation `⟨`f `, ` X `⟩` := @simplicial_map.mk _ _ _ X (simplicial_image X f) f (map_is_simplicial_onto_image X f)
+
+lemma simplicial_image_is_lift_image
+    (X : simplicial_complex α)
+    (f : α → β)
+  : (simplicial_image X f).simplices = (simplicial_map_lift ⟨f, X⟩) '' X.simplices
+:= begin
+  simp only [simplicial_image, simplicial_map_lift, set.ext_iff],
+  intro s,
+  split,
+
+  intro s_in_img,
+  simp only [set.mem_set_of] at s_in_img,
+  choose t t_in_X ft_eq_s using s_in_img,
+  simp only [set.mem_image],
+  use t, split; assumption,
+
+  intro s_in_lift,
+  simp only [set.mem_image] at s_in_lift,
+  choose t t_in_X ft_eq_s using s_in_lift,
+  simp only [set.mem_set_of],
+  use t, split; assumption,
+end
+
+lemma simplicial_image_union
+    (X Y : simplicial_complex α) [decidable_eq α]
+    (f : α → β)
+  : (simplicial_image (X ∪ Y) f).simplices = (simplicial_image X f).simplices ∪ (simplicial_image Y f).simplices
+:= begin
+  simp only [simplicial_image_is_lift_image, simplicial_map_lift, simplicial_union, set.image, set.ext_iff, set.mem_union, set.mem_set_of],
+  intro t,
+  split,
+
+  intro t_in_img_union,
+  choose s s_in_XY fs_eq_t using t_in_img_union,
+  cases s_in_XY with s_in_X s_in_Y,
+
+  left, use s, split; assumption,
+  right, use s, split; assumption,
+
+  intro t_in_union_img,
+  cases t_in_union_img with t_in_left t_in_right,
+
+  choose s s_in_X fs_eq_t using t_in_left,
+  use s, split,
+  left, assumption,
+  assumption,
+
+  choose s s_in_Y fs_eq_t using t_in_right,
+  use s, split,
+  right, assumption,
+  assumption,
 end
 
 end simplicial_map
@@ -189,6 +269,140 @@ lemma simplicial_map_on_vertices
   rw [finset.mem_coe],
   apply finset.mem_image_of_mem,
   rw [finset.mem_singleton],
+end
+
+lemma simplicial_lift_bij_implies_vertices_bij
+    (X : simplicial_complex α)
+    (Y : simplicial_complex β)
+    (f : simplicial_map X Y)
+  : set.bij_on (simplicial_map_lift f) X.simplices Y.simplices → set.bij_on f.map (vertices X) (vertices Y)
+:= begin
+  simp only [set.bij_on, set.maps_to, set.inj_on, set.surj_on, simplicial_map_lift, vertices_set_of],
+  intro lift_bij,
+  choose lift_range lift_inj lift_surj using lift_bij,
+  split,
+
+  intros x x_in_X,
+  simp only [set.mem_set_of] at x_in_X ⊢,
+  choose s s_in_X x_in_s using x_in_X,
+  specialize lift_range s_in_X,
+  use (finset.image f.map s),
+  split, assumption,
+  apply finset.mem_image_of_mem,
+  assumption,
+  
+  split,
+  intros x₁ x₁_in_X x₂ x₂_in_X fx₁_eq_fx₂,
+  simp only [set.mem_set_of] at x₁_in_X x₂_in_X,
+  rw [←vertex_iff_in_simplex, vertex_iff_singleton] at x₁_in_X x₂_in_X,
+  specialize lift_inj x₁_in_X x₂_in_X,
+  rw [←finset.singleton_inj, ←finset.image_singleton, ←finset.image_singleton] at fx₁_eq_fx₂,
+  specialize lift_inj fx₁_eq_fx₂,
+  rw [finset.singleton_inj] at lift_inj,
+  assumption,
+  
+  simp only [set.subset_def] at lift_surj ⊢,
+  intros y y_in_Y,
+  simp only [set.mem_set_of] at y_in_Y,
+  choose t t_in_Y y_in_t using y_in_Y,
+  specialize lift_surj t t_in_Y,
+  
+  simp only [set.mem_image] at lift_surj ⊢,
+  choose s s_in_X fs_eq_t using lift_surj,
+  rw [←fs_eq_t, finset.mem_image] at y_in_t,
+  choose x x_in_s fx_eq_y using y_in_t,
+  
+  use x, split,
+  simp only [set.mem_set_of],
+  use s, split; assumption,
+  assumption,
+end
+
+lemma vertices_bij_implies_simplicial_lift_maps_to
+    (X : simplicial_complex α)
+    (Y : simplicial_complex β)
+    (f : simplicial_map X Y)
+  : set.bij_on f.map (vertices X) (vertices Y) → set.maps_to (simplicial_map_lift f) X.simplices Y.simplices
+:= begin
+  simp only [set.bij_on, set.maps_to, set.inj_on, set.surj_on, simplicial_map_lift, vertices_set_of],
+  intro img_bij,
+  choose img_range img_inj img_surj using img_bij,
+  
+  intros s s_in_X,
+  by_cases s_ne : s = ∅,
+  
+  subst s_ne,
+  rw [finset.image_empty],
+  apply simplicial_complex_empty_simplex,
+  
+  simp only [finset.eq_empty_iff_forall_not_mem, not_forall, not_not] at s_ne,
+  choose x x_in_s using s_ne,
+  have x_in_X : x ∈ vertices X, from
+  begin
+    rw [vertices_set_of, set.mem_set_of],
+    use s, split; assumption,
+  end,
+  rw [vertices_set_of] at x_in_X,
+  specialize img_range x_in_X,
+  
+  simp only [set.mem_set_of] at img_range,
+  choose t t_in_Y fx_in_t using img_range,
+  apply f.is_simplicial,
+  assumption,
+end
+
+lemma vertices_bij_implies_simplicial_lift_inj
+    (X : simplicial_complex α)
+    (Y : simplicial_complex β)
+    (f : simplicial_map X Y)
+  : set.bij_on f.map (vertices X) (vertices Y) → set.inj_on (simplicial_map_lift f) X.simplices
+:= begin
+  simp only [set.bij_on, set.maps_to, set.inj_on, set.surj_on, simplicial_map_lift, vertices_set_of],
+  intro img_bij,
+  choose img_range img_inj img_surj using img_bij,
+  
+  intros s₁ s₁_in_X s₂ s₂_in_X fs₁_eq_fs₂,
+  simp only [finset.ext_iff] at fs₁_eq_fs₂ ⊢,
+
+  have s₁_ss_vert : ↑s₁ ⊆ vertices X, by { apply simplex_subset_vertices X s₁ s₁_in_X, },
+  have s₂_ss_vert : ↑s₂ ⊆ vertices X, by { apply simplex_subset_vertices X s₂ s₂_in_X, },
+
+  intro a,
+  specialize fs₁_eq_fs₂ (f.map a),
+  cases fs₁_eq_fs₂ with fs₁_ss_fs₂ fs₂_ss_fs₁,
+  split,
+
+  intro a_in_s₁,
+  have fa_in_fs₁ : f.map a ∈ finset.image f.map s₁, from
+  begin
+    apply finset.mem_image_of_mem f.map a_in_s₁,
+  end,
+  specialize fs₁_ss_fs₂ fa_in_fs₁,
+  rw [←finset.mem_coe, finset.coe_image, @set.inj_on.mem_image_iff _ _ (vertices X), finset.mem_coe] at fs₁_ss_fs₂,
+  assumption,
+  simp only [vertices_set_of, exists_prop],
+  assumption,
+  assumption,
+
+  apply set.mem_of_subset_of_mem s₁_ss_vert,
+  rw [finset.mem_coe],
+  assumption,
+
+  intro a_in_s₂,
+  have fa_in_fs₂ : f.map a ∈ finset.image f.map s₂, from
+  begin
+    apply finset.mem_image_of_mem f.map a_in_s₂,
+  end,
+  specialize fs₂_ss_fs₁ fa_in_fs₂,
+  rw [←finset.mem_coe, finset.coe_image, @set.inj_on.mem_image_iff _ _ (vertices X), finset.mem_coe] at fs₂_ss_fs₁,
+  assumption,
+  simp only [vertices_set_of, exists_prop],
+  assumption,
+  assumption,
+
+  apply set.mem_of_subset_of_mem s₂_ss_vert,
+  rw [finset.mem_coe],
+  assumption,
 end
 
 end vertices
@@ -392,7 +606,14 @@ lemma iso_inv_is_iso
     (f : simplicial_map X Y)
     (g : simplicial_map Y X)
   : is_simplicial_iso f → is_inverse_simplicial_iso f g → is_simplicial_iso g
-:= sorry
+:= begin
+  intros f_iso g_inv_f,
+  unfold is_simplicial_iso,
+  use f,
+  rw [is_inverse_simplicial_iso] at g_inv_f ⊢,
+  rw [and_comm],
+  assumption,
+end
 
 -- The composition of two isomorphisms gives an isomorphism.
 lemma iso_comp_is_iso
@@ -430,23 +651,126 @@ lemma iso_comp_is_iso
   assumption,
 end
 
-lemma iso_is_injective
+lemma iso_is_injective_vertices
     {X : simplicial_complex α}
     {Y : simplicial_complex β}
     (f : simplicial_map X Y)
     (f_iso : is_simplicial_iso f)
   : set.inj_on f.map (vertices X)
 := begin
-  sorry
+  unfold is_simplicial_iso at f_iso,
+  choose g g_inv_f using f_iso,
+  unfold is_inverse_simplicial_iso at g_inv_f,
+  choose fg_id gf_id using g_inv_f,
+
+  simp only [function.funext_iff, set.restrict_eq_restrict_iff, set.eq_on] at fg_id,
+  unfold set.inj_on,
+  intros x₁ x₁_in_X x₂ x₂_in_X fx₁_eq_fx₂,
+
+  have fgx₁_eq_x₁ : (f.comp g).map x₁ = id x₁, from
+  begin
+    specialize fg_id x₁_in_X,
+    assumption,
+  end,
+
+  have fgx₂_eq_x₂ : (f.comp g).map x₂ = id x₂, from
+  begin
+    specialize fg_id x₂_in_X,
+    assumption,
+  end,
+
+  simp only [simplicial_map.comp, function.comp_apply] at fgx₁_eq_x₁ fgx₂_eq_x₂,
+  simp only [fx₁_eq_fx₂, fgx₂_eq_x₂, id.def] at fgx₁_eq_x₁,
+  symmetry,
+  assumption,
 end
 
-lemma iso_is_surjective
+lemma iso_is_injective_simplices
+    {X : simplicial_complex α}
+    {Y : simplicial_complex β}
+    (f : simplicial_map X Y)
+    (f_iso : is_simplicial_iso f)
+  : ∀ s ∈ X.simplices, set.inj_on f.map ↑s
+:= begin
+  intros s s_in_X,
+  simp only [set.inj_on],
+  intros x₁ x₁_in_s x₂ x₂_in_s fx₁_eq_fx₂,
+
+  unfold is_simplicial_iso at f_iso,
+  choose g gf_inv using f_iso,
+  unfold is_inverse_simplicial_iso at gf_inv,
+  choose gf_id fg_id using gf_inv,
+
+  simp only [set.restrict_eq_restrict_iff, set.eq_on, simplicial_map.comp, function.comp_apply] at gf_id,
+  have x₁_in_X : x₁ ∈ vertices X, from
+  begin
+    rw [vertex_iff_in_simplex],
+    use s, split; assumption,
+  end,
+
+  have x₂_in_X : x₂ ∈ vertices X, from
+  begin
+    rw [vertex_iff_in_simplex],
+    use s, split; assumption,
+  end,
+
+  have gfx₁_eq_x₁ : g.map (f.map x₁) = x₁, from
+  begin
+    specialize gf_id x₁_in_X,
+    rw [id.def] at gf_id,
+    assumption,
+  end,
+
+  have gfx₂_eq_x₂ : g.map (f.map x₂) = x₂, from
+  begin
+    specialize gf_id x₂_in_X,
+    rw [id.def] at gf_id,
+    assumption,
+  end,
+
+  have gfx₁_eq_gfx₂ : g.map (f.map x₁) = g.map (f.map x₂), from
+  begin
+    apply congr_arg g.map,
+    assumption,
+  end,
+
+  rw [gfx₁_eq_x₁, gfx₂_eq_x₂] at gfx₁_eq_gfx₂,
+  assumption,
+end
+
+lemma iso_is_surjective_vertices
     {X : simplicial_complex α}
     {Y : simplicial_complex β}
     (f : simplicial_map X Y)
     (f_iso : is_simplicial_iso f)
   : set.surj_on f.map (vertices X) (vertices Y)
-:= sorry
+:= begin
+  unfold is_simplicial_iso at f_iso,
+  choose g g_inv_f using f_iso,
+  unfold is_inverse_simplicial_iso at g_inv_f,
+  choose fg_id gf_id using g_inv_f,
+
+  simp only [function.funext_iff, set.restrict_eq_restrict_iff, set.eq_on] at gf_id,
+  simp only [set.surj_on, set.subset_def, set.mem_image],
+  intros x x_in_Y,
+
+  specialize gf_id x_in_Y,
+  simp only [simplicial_map.comp, function.comp_apply] at gf_id,
+  use (g.map x), split,
+
+  rw [vertex_iff_in_simplex] at x_in_Y ⊢,
+  choose s s_in_Y x_in_s using x_in_Y,
+
+  use (finset.image g.map s), split,
+  apply g.is_simplicial,
+  assumption,
+  apply finset.mem_image_of_mem,
+
+  assumption,
+
+  rw [id.def] at gf_id,
+  assumption,
+end
 
 -- Defining isomorphy between simplicial complexes.
 @[simp]
@@ -457,27 +781,181 @@ def is_simplicially_iso
 := ∃ (f : simplicial_map X Y), is_simplicial_iso f
 infixr ` ≅ `:50 := is_simplicially_iso
 
+lemma simplicial_iso_implies_lift_bij
+    (X : simplicial_complex α)
+    (Y : simplicial_complex β)
+    (f : simplicial_map X Y)
+  : is_simplicial_iso f → Y.simplices = (simplicial_map_lift f) '' X.simplices
+:= begin
+  intro f_iso,
+  unfold is_simplicial_iso at f_iso,
+  choose g g_inv_f using f_iso,
+  unfold is_inverse_simplicial_iso at g_inv_f,
+  choose fg_id gf_id using g_inv_f,
+
+  rw [set.ext_iff],
+  intro t,
+  split,
+
+  intro t_in_Y,
+  simp only [simplicial_map_lift, set.mem_image],
+  use (finset.image g.map t),
+  split,
+  apply g.is_simplicial,
+  assumption,
+
+  simp only [←finset.coe_inj, finset.coe_image],
+  rw [←set.image_comp],
+  conv_rhs {
+    rw [←set.image_id ↑t],
+  },
+  apply set.eq_on.image_eq,
+  simp only [function.funext_iff, set.restrict_eq_restrict_iff, simplicial_map.comp] at gf_id,
+  have t_in_vert : ↑t ⊆ vertices Y, by { apply simplex_subset_vertices Y t t_in_Y, },
+  apply set.eq_on.mono t_in_vert,
+  assumption,
+
+  intro t_in_lift,
+  simp only [simplicial_map_lift, set.mem_image] at t_in_lift,
+  choose s s_in_X fs_eq_t using t_in_lift,
+  subst fs_eq_t,
+  apply f.is_simplicial,
+  assumption,
+end
+
+lemma simplicial_iso_vertices
+    (X : simplicial_complex α)
+    (Y : simplicial_complex β)
+    (f : simplicial_map X Y)
+  : is_simplicial_iso f → vertices Y = f.map '' vertices X
+:= begin
+  intro f_iso,
+  unfold is_simplicial_iso at f_iso,
+  choose g gf_inv using f_iso,
+  unfold is_inverse_simplicial_iso at gf_inv,
+  simp only [set.restrict_eq_restrict_iff, set.eq_on, simplicial_map.comp, function.comp_app, id.def] at gf_inv,
+  choose gf_id fg_id using gf_inv,
+
+  rw [set.ext_iff],
+  intro x,
+  split,
+
+  intro x_in_Y,
+  specialize fg_id x_in_Y,
+  rw [set.mem_image],
+  use (g.map x), split,
+
+  rw [vertex_iff_singleton] at x_in_Y ⊢,
+  rw [←finset.image_singleton],
+  apply g.is_simplicial,
+  assumption,
+
+  assumption,
+
+  intro x_in_img,
+  rw [set.mem_image] at x_in_img,
+  choose y y_in_X fy_eq_x using x_in_img,
+  rw [vertex_iff_singleton] at y_in_X ⊢,
+  rw [←fy_eq_x, ←finset.image_singleton],
+  apply f.is_simplicial,
+  assumption,
+end
+
+noncomputable
 instance is_simplicially_iso.fintype
     (X : simplicial_complex α) [fintype X.simplices]
     (Y : simplicial_complex β)
     (X_iso_Y : X ≅ Y)
   : fintype Y.simplices
-:= sorry
+:= begin
+  unfold is_simplicially_iso at X_iso_Y,
+  choose f f_iso using X_iso_Y,
+  rw [simplicial_iso_implies_lift_bij X Y f f_iso],
+
+  apply set.fintype_image,
+end
+
+lemma simplicial_iso_preserves_simplex_dim
+    {X : simplicial_complex α}
+    {Y : simplicial_complex β}
+    (f : simplicial_map X Y)
+    (f_iso : is_simplicial_iso f)
+  : ∀ s ∈ X.simplices, dim s = dim (finset.image f.map s)
+:= begin
+  intros s s_in_X,
+  unfold dim,
+  apply congr_arg (λ (z : ℤ), z - 1),
+  symmetry,
+  rw [nat.cast_inj, finset.card_image_iff],
+  apply iso_is_injective_simplices f f_iso s s_in_X,
+end
 
 lemma simplicial_iso_preserves_dim
     (X : simplicial_complex α) [X_fin : fintype X.simplices]
     (Y : simplicial_complex β)
     (X_iso_Y : X ≅ Y)
-  : @dim_of_complex α X = @dim_of_complex β Y (@is_simplicially_iso.fintype α β _ _ X X_fin Y X_iso_Y)
-:= sorry
+  : @dim_of_complex α X X_fin = @dim_of_complex β Y (@is_simplicially_iso.fintype α β _ _ X X_fin Y X_iso_Y)
+:= begin
+  unfold is_simplicially_iso at X_iso_Y,
+  choose f f_iso using X_iso_Y,
+  simp only [dim_of_complex],
+  
+  rw [le_antisymm_iff],
+  split,
+
+  -- dim X ≤ dim Y case.
+  rw [finset.max'_le_iff],
+  intros n n_X_dim,
+  rw [finset.mem_image] at n_X_dim,
+  choose s s_in_X s_dim_n using n_X_dim,
+  rw [set.mem_to_finset] at s_in_X,
+  rw [←s_dim_n],
+
+  apply finset.le_max',
+  rw [simplicial_iso_preserves_simplex_dim f f_iso s s_in_X, finset.mem_image],
+  use (finset.image f.map s),
+  split,
+
+  rw [set.mem_to_finset],
+  apply f.is_simplicial,
+  assumption,
+
+  refl,
+
+  -- dim Y ≤ dim X case.
+  rw [finset.max'_le_iff],
+  intros m m_Y_dim,
+  rw [finset.mem_image] at m_Y_dim,
+  choose t t_in_Y t_dim_m using m_Y_dim,
+  rw [set.mem_to_finset] at t_in_Y,
+  rw [←t_dim_m],
+
+  let f_iso' := f_iso,
+  unfold is_simplicial_iso at f_iso',
+  choose g gf_inv using f_iso',
+  have g_iso : is_simplicial_iso g, from
+  begin
+    apply iso_inv_is_iso f g f_iso gf_inv,
+  end,
+
+  apply finset.le_max',
+  rw [simplicial_iso_preserves_simplex_dim g g_iso t t_in_Y, finset.mem_image],
+  use (finset.image g.map t),
+  split,
+
+  rw [set.mem_to_finset],
+  apply g.is_simplicial,
+  assumption,
+
+  refl,
+end
 
 -- Being simplicially isomorphic is an equivalence relation.
 @[refl]
 lemma simplicial_iso_refl
     (X : simplicial_complex α)
   : X ≅ X
-:=
-begin
+:= begin
   unfold is_simplicially_iso,
   use id_simplicial_map X,
   apply id_is_simplicial_iso,
@@ -544,9 +1022,12 @@ lemma simplicial_iso_preserves_equiv
     assumption,
   end,
 
-  use ⟨id, id_simplicial_X⟩,
+  set id_X := simplicial_map.mk id id_simplicial_X,
+  use id_X,
   unfold is_simplicial_iso,
-  use ⟨id, id_simplicial_Y⟩,
+
+  set id_Y := simplicial_map.mk id id_simplicial_Y,
+  use id_Y,
 
   unfold is_inverse_simplicial_iso,
   split; simp only[simplicial_map.comp];
@@ -554,50 +1035,26 @@ lemma simplicial_iso_preserves_equiv
   simp only[id_simplicial_map],
 end
 
-lemma empty_iso_empty
-  : @empty_sc α ≅ @empty_sc β
-:= sorry
-
-lemma simplicial_union_iso
-    (X Y : simplicial_complex α)
-    (Z W : simplicial_complex β)
-  : X ≅ Z → Y ≅ W → X ∪ Y ≅ Z ∪ W
-:= sorry
-
-lemma simplicial_union_iso_left
+lemma simplicial_iso_preserves_subcomplex_image
     (X Y Z : simplicial_complex α)
-  : X ≅ Y → X ∪ Z ≅ Y ∪ Z
+    (f : simplicial_map Y Z)
+    (f_iso : is_simplicial_iso f)
+  : X ⊆ Y → simplicial_image X f.map ⊆ Z
 := begin
-  intro X_iso_Y,
-  apply simplicial_union_iso,
-  assumption,
-  apply simplicial_iso_refl,
+  intro X_sub_Y,
+  simp only [is_subcomplex] at X_sub_Y ⊢,
+
+  rw [simplicial_iso_implies_lift_bij Y Z f f_iso],
+  simp only [simplicial_map_lift, set.image],
+  simp only [set.subset_def] at X_sub_Y ⊢,
+
+  intros t t_in_fX,
+  simp only [set.mem_set_of] at t_in_fX ⊢,
+  choose s s_in_X fs_eq_t using t_in_fX,
+  specialize X_sub_Y s s_in_X,
+
+  use s, split; assumption,
 end
-
-lemma simplicial_union_iso_right
-    (X Y Z : simplicial_complex α)
-  : X ≅ Y → Z ∪ X ≅ Z ∪ Y
-:= begin
-  intro X_iso_Y,
-  apply simplicial_union_iso,
-  apply simplicial_iso_refl,
-  assumption,
-end
-
-lemma simplicial_iso_preserves_subcomplex
-    (X Y Z W : simplicial_complex α)
-  : X ≅ Z → Y ≅ W → X ⊆ Y → Z ⊆ W
-:= sorry
-
-lemma simplicial_union_eq_left_iff_subcomplex
-    (X Y : simplicial_complex α)
-  : (X ∪ Y).simplices = X.simplices ↔ Y ⊆ X
-:= sorry
-
-lemma simplicial_union_eq_right_iff_subcomplex
-    (X Y : simplicial_complex α)
-  : (X ∪ Y).simplices = Y.simplices ↔ X ⊆ Y
-:= sorry
 
 end isomorphism
 
@@ -610,39 +1067,106 @@ section coercion
 variables [decidable_eq α] [decidable_eq β] [decidable_eq γ]
 
 -- Define as coercion on types that lifts to simplicial map.
--- structure simplicial_coe'
---     (α : Type*) [decidable_eq α]
---     (β : Type*) [decidable_eq β]
--- := mk :: (coe : α → β)
---          (injective : set.inj_on coe (vertices X))
---          (iso_onto_image : ∀ X : simplicial_complex α, X ≅ simplicial_image X coe injective)
-
 structure simplicial_coe
     (X : simplicial_complex α)
-    (β : Type*) [decidable_eq β]
+    (β : Type*)
 := mk :: (coe : α → β)
          (injective : set.inj_on coe (vertices X))
-notation φ `[` X `]` := simplicial_image X φ.coe φ.injective
+notation φ `[` X `]` := simplicial_image X φ.coe
+
+def simplicial_coe.simplicial_map
+    {X : simplicial_complex α}
+    (φ : simplicial_coe X β)
+  : simplicial_map X (φ[X])
+:= simplicial_map.mk φ.coe (map_is_simplicial_onto_image X φ.coe)
 
 instance simplicial_coe.fintype
     (X : simplicial_complex α) [fintype X.simplices]
     (φ : simplicial_coe X β)
   : fintype (φ[X]).simplices
-:= sorry
+:= begin
+  rw [simplicial_image_is_lift_image],
+  apply set.fintype_image,
+end
 
-lemma simplicial_coe.iso_onto_image
+lemma simplicial_coe_inv_is_simplicial
+    [nonempty α]
     {X : simplicial_complex α}
     (φ : simplicial_coe X β)
-  : X ≅ φ[X]
-:= sorry
+  : is_simplicial_map (φ[X]) X (function.inv_fun_on φ.coe (vertices X))
+:= begin
+  simp only [is_simplicial_map, simplicial_image],
+  intros t t_in_coe,
+  simp only [set.mem_set_of] at t_in_coe,
+  choose s s_in_X coe_s_t using t_in_coe,
+
+  rw [←coe_s_t],
+  have inv_id : finset.image (function.inv_fun_on φ.coe (vertices X)) (finset.image φ.coe s) = s, from
+  begin
+    simp only [←finset.coe_inj, finset.coe_image],
+    apply set.inj_on.inv_fun_on_image,
+    apply φ.injective,
+    apply simplex_subset_vertices,
+    assumption,
+  end,
+  rw [inv_id],
+  assumption,
+end
+
+noncomputable
+def simplicial_coe_inv
+    [nonempty α]
+    {X : simplicial_complex α}
+    (φ : simplicial_coe X β)
+  : simplicial_map (φ[X]) X
+:= simplicial_map.mk (function.inv_fun_on φ.coe (vertices X)) (simplicial_coe_inv_is_simplicial φ)
+notation φ`⁻ᶜ` := simplicial_coe_inv φ
+
+lemma coe_inv_is_inverse_simplicial_iso
+    [nonempty α]
+    {X : simplicial_complex α}
+    (φ : simplicial_coe X β)
+  : is_inverse_simplicial_iso (simplicial_map.mk φ.coe (map_is_simplicial_onto_image X φ.coe)) (φ⁻ᶜ)
+:= begin
+  simp only [is_inverse_simplicial_iso, simplicial_map.comp, set.restrict_eq_restrict_iff],
+  split,
+
+  apply set.inj_on.left_inv_on_inv_fun_on,
+  apply φ.injective,
+  
+  simp only [set.eq_on, id.def],
+  intros y y_in_coe,
+  apply function.inv_fun_on_eq,
+  rw [simplicial_image_vertices, set.mem_image] at y_in_coe,
+  choose x x_in_X coe_x_y using y_in_coe,
+  use x, split; assumption,
+end
 
 lemma coe_is_iso
+    [nonempty α]
     (X : simplicial_complex α)
     (φ : simplicial_coe X β)
   : is_simplicial_iso (@simplicial_map.mk α β _ X (φ[X]) φ.coe (by { apply map_is_simplicial_onto_image, }))
-:= sorry
+:= begin
+  unfold is_simplicial_iso,
+  use (@simplicial_coe_inv _ _ _ _ _ X φ),
+  apply coe_inv_is_inverse_simplicial_iso,
+end
+
+lemma simplicial_coe.iso_onto_image
+    [nonempty α]
+    {X : simplicial_complex α}
+    (φ : simplicial_coe X β)
+  : X ≅ φ[X]
+:= begin
+  unfold is_simplicially_iso,
+  use φ.coe,
+  apply map_is_simplicial_onto_image,
+  apply coe_is_iso,  
+end
 
 lemma coe_preserves_iso
+    [nonempty α]
     (X Y : simplicial_complex α)
     (φ : simplicial_coe X β)
     (ψ : simplicial_coe Y β)
@@ -691,7 +1215,7 @@ lemma coe_comp_image
     (X : simplicial_complex α)
     (φ : simplicial_coe X β)
     (ψ : simplicial_coe (φ[X]) γ)
-  : (simplicial_image X (ψ.coe ∘ φ.coe) (coe_comp_is_injective φ ψ)).simplices = (simplicial_image (φ[X]) ψ.coe ψ.injective).simplices
+  : (simplicial_image X (ψ.coe ∘ φ.coe)).simplices = (simplicial_image (φ[X]) ψ.coe).simplices
 := begin
   dsimp only [simplicial_image, simplicial_complex.simplices],
   rw [set.ext_iff],
@@ -738,7 +1262,10 @@ lemma coe_restrict_is_injective
     (φ : simplicial_coe X β)
     (Y_subcomp_X : vertices Y ⊆ vertices X)
   : set.inj_on φ.coe (vertices Y)
-:= sorry
+:= begin
+  apply set.inj_on.mono Y_subcomp_X,
+  apply φ.injective,
+end
 
 @[simp]
 def simplicial_coe.restrict
@@ -748,7 +1275,7 @@ def simplicial_coe.restrict
     (Y_subcomp_X : vertices Y ⊆ vertices X)
   : simplicial_coe Y β
 := simplicial_coe.mk φ.coe (coe_restrict_is_injective X Y φ Y_subcomp_X)
-notation φ `[` Y `; ` H `]` := simplicial_image Y (simplicial_coe.restrict φ Y H).coe (simplicial_coe.restrict φ Y H).injective
+notation φ `[` Y `; ` H `]` := simplicial_image Y (simplicial_coe.restrict φ Y H).coe
 
 def simplicial_coe.restrict_coe
     {X Y : simplicial_complex α}
@@ -763,7 +1290,7 @@ def simplicial_map.coe
     (f : simplicial_map X Y)
     (f_iso : is_simplicial_iso f)
   : simplicial_coe X β
-:= simplicial_coe.mk f.map (iso_is_injective f f_iso)
+:= simplicial_coe.mk f.map (iso_is_injective_vertices f f_iso)
 
 -- Coercion on images.
 --  g[Y] = X → φ[X]
@@ -777,19 +1304,40 @@ def simplicial_coe_on_image
     (Y_img_X : Y.simplices = simplicial_map_lift f '' X.simplices)
     (φ : simplicial_coe Y γ)
   : simplicial_coe X γ
-:= simplicial_coe.mk (φ.coe ∘ f.map) sorry
+:= simplicial_coe.mk
+    (φ.coe ∘ f.map)
+    (begin
+      apply set.inj_on.comp φ.injective,
+      apply (f.coe f_iso).injective,
+
+      unfold set.maps_to,
+      intros x x_in_X,
+      simp only [vertex_iff_singleton, Y_img_X, simplicial_map_lift, set.image, set.mem_set_of],
+      use {x}, split,
+
+      rw [←vertex_iff_singleton],
+      assumption,
+
+      apply finset.image_singleton,
+    end)
 
 
 lemma simplicial_coe_union_simplices
     (X Y : simplicial_complex α)
     (φ : simplicial_coe (X ∪ Y) β)
-  : φ[X ∪ Y].simplices = (φ[X; sorry] ∪ φ[Y; sorry]).simplices
-:= sorry
+  : φ[X ∪ Y].simplices =
+      (φ[X; by { apply is_subcomplex_vertices, apply subcomplex_simplicial_union_left, }]
+        ∪ φ[Y; by { apply is_subcomplex_vertices, apply subcomplex_simplicial_union_right, }]).simplices
+:= begin
+  apply simplicial_image_union,
+end
 
 lemma simplicial_coe_union
     (X Y : simplicial_complex α)
     (φ : simplicial_coe (X ∪ Y) β)
-  : φ[X ∪ Y] ≅ φ[X; sorry] ∪ φ[Y; sorry]
+  : φ[X ∪ Y] ≅
+      (φ[X; by { apply is_subcomplex_vertices, apply subcomplex_simplicial_union_left, }]
+        ∪ φ[Y; by { apply is_subcomplex_vertices, apply subcomplex_simplicial_union_right, }])
 := begin
   apply simplicial_iso_preserves_equiv,
   apply simplicial_coe_union_simplices,
@@ -1207,69 +1755,25 @@ lemma simplex_disjoint_distr_inter
   repeat { rw [finset.inter_product] },
 end
 
+lemma simplex_disjoint_card
+    (s t : finset α)
+  : (s ⊔ₛ t).card = s.card + t.card
+:= begin
+  simp only [simplex_disjoint_union],
+  set s₀ : finset (α × ℕ) := s ×ˢ {0},
+  set t₁ : finset (α × ℕ) := t ×ˢ {1},
+
+  have card_disj : (s₀ ∪ t₁).card = s₀.card + t₁.card, from
+  begin
+    apply finset.card_union_eq,
+    simp only [s₀, t₁, finset.disjoint_product, finset.disjoint_singleton],
+    right,
+    apply nat.zero_ne_one,
+  end,
+  simp only [card_disj, s₀, t₁, finset.card_product, finset.card_singleton, mul_one],
+end
+
 -- Define simplicial join.
-@[simp]
-def simplicial_join'
-    (X Y : simplicial_complex α)
-  : simplicial_complex (α × ℕ) 
-:= simplicial_complex.mk
-    (⋃ (s ∈ X.simplices), ⋃ (t ∈ Y.simplices), {s ⊔ₛ t})
-    (begin
-      rw [set.nonempty_coe_sort, set.nonempty_def],
-      use (∅ : finset (α × ℕ)),
-      rw [set.mem_Union],
-      use (∅ : finset α),
-      rw [set.mem_Union],
-      use simplicial_complex_empty_simplex X,
-      rw [set.mem_Union],
-      use (∅ : finset α),
-      rw [set.mem_Union],
-      use simplicial_complex_empty_simplex Y,
-      have H_empty : (∅ : finset (α × ℕ)) = (∅ : finset α) ⊔ₛ (∅ : finset α), from
-      begin
-        symmetry,
-        rw [simplex_disjoint_empty],
-        split; refl,
-      end,
-      rw [←H_empty],
-      sorry,
-    end)
-    (begin
-      simp only[is_subset_closed],
-      intros s s_in_XY t t_sset_s,
-      rw [set.mem_Union] at *,
-
-      choose z s_in_XY using s_in_XY,
-      rw [set.mem_Union] at s_in_XY,
-      choose Hz s_in_XY using s_in_XY,
-      rw [set.mem_Union] at s_in_XY,
-      choose w s_in_XY using s_in_XY,
-      rw [set.mem_Union] at s_in_XY,
-      choose Hw s_eq_zw using s_in_XY,
-      rw [set.mem_singleton_iff] at s_eq_zw,
-      rw [s_eq_zw, simplex_disjoint_subset_sep] at t_sset_s,
-      choose zt wt t_eq_zw using t_sset_s,
-      choose t_eq_zw zt_sset_z wt_sset_w using t_eq_zw,
-
-      use zt,
-      rw [set.mem_Union],
-      have Hzt : zt ∈ X.simplices, from
-      begin
-        apply X.subset_closed z; assumption,
-      end,
-      use Hzt,
-      rw [set.mem_Union],
-      use wt,
-      rw [set.mem_Union],
-      have Hwt : wt ∈ Y.simplices, from
-      begin
-        apply Y.subset_closed w; assumption,
-      end,
-      use Hwt,
-      rw [set.mem_singleton_iff],
-      assumption,
-    end)
-
 @[simp]
 def simplicial_join
     (X Y : simplicial_complex α)
@@ -1305,14 +1809,41 @@ def simplicial_join
     end)
 infixl ` ⋆ `:70 := simplicial_join
 
+lemma simplicial_join_as_union
+    (X Y : simplicial_complex α)
+  : (X ⋆ Y).simplices = ⋃ (s ∈ X.simplices), ⋃ (t ∈ Y.simplices), {s ⊔ₛ t}
+:= begin
+  simp only [simplicial_join, set.ext_iff, set.mem_Union, set.mem_set_of, set.mem_singleton_iff],
+  intro x,
+  split,
+
+  intro x_in_join,
+  choose s s_in_X t t_in_Y st_eq_x using x_in_join,
+  use s, split, assumption,
+  use t, split, assumption,
+  symmetry, assumption,
+
+  intro x_in_union,
+  choose s s_in_X t t_in_Y st_eq_x using x_in_union,
+  use s, split, assumption,
+  use t, split, assumption,
+  symmetry, assumption,
+end
+
 -- Establish basic algebraic properties about joins.
 instance simplicial_join.fintype
     (X : simplicial_complex α) [fintype X.simplices]
     (Y : simplicial_complex α) [fintype Y.simplices]
   : fintype (X ⋆ Y).simplices
 := begin
-  simp only[simplicial_join, simplicial_complex.simplices, simplex_disjoint_union],
-  sorry, -- TODO: set.finite.dependent,
+  rw [simplicial_join_as_union],
+  apply set.fintype_bUnion,
+  intros s s_in_X,
+
+  apply set.fintype_bUnion,
+  intros t t_in_Y,
+
+  apply unique.fintype,
 end
 
 lemma simplicial_join_sep
@@ -1587,7 +2118,173 @@ lemma simplicial_join_mem_vertices
     split; assumption, }
 end
 
+def simplicial_join_iso_map
+    (f g : α → β)
+  : α × ℕ → β × ℕ
+:= λ x : α × ℕ, if (x.snd = 0) then (f x.fst, x.snd) else (g x.fst, x.snd)
+
+lemma simplicial_join_iso_simplicial
+    (X Y : simplicial_complex α)
+    (Z W : simplicial_complex β)
+    (f : simplicial_map X Z)
+    (g : simplicial_map Y W)
+  : is_simplicial_map (X ⋆ Y) (Z ⋆ W) (simplicial_join_iso_map f.map g.map)
+:= begin
+  unfold is_simplicial_map,
+  intros s s_in_XY,
+
+  rw [simplicial_join_mem] at *,
+  choose t Ht u Hu s_eq_tu using s_in_XY,
+
+  use (finset.image f.map t), split,
+  apply f.is_simplicial,
+  assumption,
+
+  use (finset.image g.map u), split,
+  apply g.is_simplicial,
+  assumption,
+
+  rw [s_eq_tu],
+  simp only[simplex_disjoint_union],
+  rw [finset.image_union],
+
+  rw [finset.ext_iff],
+  intro x,
+  split,
+  { intro x_in_f,
+    rw [finset.mem_union] at *,
+    cases x_in_f,
+    
+    left,
+    rw [finset.mem_product],
+    rw [finset.mem_image] at *,
+    choose y y_in_t0 using x_in_f,
+    cases y_in_t0 with y_in_t0 fy_x,
+
+    use y.fst,
+    rw [finset.mem_product] at y_in_t0,
+    cases y_in_t0 with y_in_t0 y_0,
+    split,
+    assumption,
+
+    simp only [simplicial_join_iso_map] at fy_x,
+    revert fy_x,
+    split_ifs,
+    
+    intro y0_x,
+    rw [←y0_x],
+    
+    rw [finset.mem_singleton] at y_0,
+    contradiction,
+    
+    simp only [simplicial_join_iso_map] at fy_x,
+    revert fy_x,
+    split_ifs,
+    
+    intro y0_x,
+    rw [finset.mem_singleton, ←y0_x],
+    
+    rw [finset.mem_product] at y_in_t0,
+    cases y_in_t0 with y_in_t0 y_0,
+    rw [finset.mem_singleton] at y_0,
+    assumption,
+    
+    intro fy_x,
+    rw [prod.eq_iff_fst_eq_snd_eq] at fy_x,
+    cases fy_x with fy_x_fst fy_x_snd,
+    simp at fy_x_snd,
+    rw [finset.mem_singleton, ←fy_x_snd],
+    finish,
+    
+    simp only [finset.mem_image, simplicial_join_iso_map] at x_in_f,
+    choose y y_in_u fy_eq_x using x_in_f,
+    revert fy_eq_x,
+    split_ifs,
+    
+    rw [finset.mem_product, finset.mem_singleton] at y_in_u,
+    choose y_in_u y_one using y_in_u,
+    have contra : y.snd ≠ 0, by omega,
+    contradiction,
+    
+    intro gy_eq_x,
+    simp only [prod.ext_iff, prod.fst, prod.snd] at gy_eq_x,
+    choose gy_eq_x x_one using gy_eq_x,
+    rw [finset.mem_product, finset.mem_singleton] at y_in_u,
+    choose y_in_u y_one using y_in_u,
+    right,
+    rw [finset.mem_product, finset.mem_image],
+    split,
+    use y.fst, split,
+    assumption,
+    assumption,
+    rw [finset.mem_singleton, ←x_one],
+    assumption, },
+
+  { intro x_in_f_prod,
+    rw [finset.mem_union] at *,
+    cases x_in_f_prod,
+    
+    left,
+    rw [finset.mem_product] at x_in_f_prod,
+    cases x_in_f_prod with x_in_fxz x0,
+    rw [finset.mem_image] at *,
+    choose y y_in_t fxz_y using x_in_fxz,
+    
+    use (y, 0),
+    split,
+
+    rw [finset.mem_product],
+    simp,
+    assumption,
+    
+    simp only [simplicial_join_iso_map],
+    split_ifs,
+    
+    rw [prod.eq_iff_fst_eq_snd_eq],
+    split,
+    assumption,
+    rw [finset.mem_singleton] at x0,
+    rw [x0],
+    
+    rw [prod.eq_iff_fst_eq_snd_eq],
+    split,
+    assumption,
+    rw [finset.mem_singleton] at x0,
+    rw [x0],
+    
+    right,
+    rw [finset.mem_product] at x_in_f_prod,
+    cases x_in_f_prod with x_in_fyw x1,
+    rw [finset.mem_singleton] at x1,
+    rw [finset.mem_image] at *,
+    choose y y_in_u fyw_y using x_in_fyw,
+    
+    use (y, 1),
+    split,
+    
+    rw [finset.mem_product],
+    split,
+    assumption,
+    simp,
+    
+    simp only [simplicial_join_iso_map],
+    split_ifs,
+    
+    finish,
+    
+    rw [prod.eq_iff_fst_eq_snd_eq],
+    split,
+    assumption,
+    rw [x1], }
+end
+
+def simplicial_join_iso_inverse_map
+    (f g : β → α)
+  : β × ℕ → α × ℕ
+:= λ x : β × ℕ, if (x.snd = 0) then (f x.fst, x.snd) else (g x.fst, x.snd)
+
 -- TODO: Fix the proofs that f, g are simplicial.
+--       Perhaps, move the function def's outside + proofs.
 lemma simplicial_join_iso
     (X Y : simplicial_complex α)
     (Z W : simplicial_complex β)
@@ -1605,308 +2302,23 @@ lemma simplicial_join_iso
   cases fxz_inv_gzx with gzx_fxz_id fxz_gzx_id,
   cases fyw_inv_gwy with gwy_fyw_id fyw_gwy_id,
 
-  let f : α × ℕ → β × ℕ :=
-    λ x : α × ℕ, if (x.snd = 0) then (f_xz.map x.fst, x.snd) else (f_yw.map x.fst, x.snd),
-
-  have f_simplicial : is_simplicial_map (X ⋆ Y) (Z ⋆ W) f, by sorry,--from
-  -- begin
-  --   unfold is_simplicial_map,
-  --   intros s s_in_XY,
-
-  --   rw [simplicial_join_mem] at *,
-  --   choose t Ht u Hu s_eq_tu using s_in_XY,
-
-  --   use (finset.image f_xz.map t), split,
-  --   apply f_xz.is_simplicial,
-  --   assumption,
-
-  --   use (finset.image f_yw.map u), split,
-  --   apply f_yw.is_simplicial,
-  --   assumption,
-
-  --   rw [s_eq_tu],
-  --   simp only[simplex_disjoint_union],
-  --   rw [finset.image_union],
-
-  --   rw [finset.ext_iff],
-  --   intro x,
-  --   split,
-  --   { intro x_in_f,
-  --     rw [finset.mem_union] at *,
-  --     cases x_in_f,
-      
-  --     left,
-  --     rw [finset.mem_product],
-  --     rw [finset.mem_image] at *,
-  --     choose y y_in_t0 using x_in_f,
-  --     cases y_in_t0 with y_in_t0 fy_x,
-
-  --     use y.fst,
-  --     rw [finset.mem_product] at y_in_t0,
-  --     cases y_in_t0 with y_in_t0 y_0,
-  --     split,
-  --     assumption,
-
-  --     simp only[f] at fy_x,
-  --     revert fy_x,
-  --     split_ifs,
-      
-  --     intro y0_x,
-  --     rw [←y0_x],
-      
-  --     rw [finset.mem_singleton] at y_0,
-  --     contradiction,
-      
-  --     simp only[f] at fy_x,
-  --     revert fy_x,
-  --     split_ifs,
-      
-  --     intro y0_x,
-  --     rw [finset.mem_singleton, ←y0_x],
-      
-  --     rw [finset.mem_product] at y_in_t0,
-  --     cases y_in_t0 with y_in_t0 y_0,
-  --     rw [finset.mem_singleton] at y_0,
-  --     assumption,
-      
-  --     intro fy_x,
-  --     rw [prod.eq_iff_fst_eq_snd_eq] at fy_x,
-  --     cases fy_x with fy_x_fst fy_x_snd,
-  --     simp at fy_x_snd,
-  --     rw [finset.mem_singleton, ←fy_x_snd],
-  --     finish,
-      
-  --     sorry, },
-  --   { intro x_in_f_prod,
-  --     rw [finset.mem_union] at *,
-  --     cases x_in_f_prod,
-      
-  --     left,
-  --     rw [finset.mem_product] at x_in_f_prod,
-  --     cases x_in_f_prod with x_in_fxz x0,
-  --     rw [finset.mem_image] at *,
-  --     choose y y_in_t fxz_y using x_in_fxz,
-      
-  --     use (y, 0),
-  --     split,
-
-  --     rw [finset.mem_product],
-  --     simp,
-  --     assumption,
-      
-  --     simp only[f],
-  --     split_ifs,
-      
-  --     rw [prod.eq_iff_fst_eq_snd_eq],
-  --     split,
-  --     assumption,
-  --     rw [finset.mem_singleton] at x0,
-  --     rw [x0],
-      
-  --     rw [prod.eq_iff_fst_eq_snd_eq],
-  --     split,
-  --     assumption,
-  --     rw [finset.mem_singleton] at x0,
-  --     rw [x0],
-      
-  --     right,
-  --     rw [finset.mem_product] at x_in_f_prod,
-  --     cases x_in_f_prod with x_in_fyw x1,
-  --     rw [finset.mem_singleton] at x1,
-  --     rw [finset.mem_image] at *,
-  --     choose y y_in_u fyw_y using x_in_fyw,
-      
-  --     use (y, 1),
-  --     split,
-      
-  --     rw [finset.mem_product],
-  --     split,
-  --     assumption,
-  --     simp,
-      
-  --     simp only[f],
-  --     split_ifs,
-      
-  --     finish,
-      
-  --     rw [prod.eq_iff_fst_eq_snd_eq],
-  --     split,
-  --     assumption,
-  --     rw [x1], }
-  -- end,
-
   let fs : simplicial_map (X ⋆ Y) (Z ⋆ W) :=
-    simplicial_map.mk f f_simplicial,
-
-  let g : β × ℕ → α × ℕ :=
-    λ x : β × ℕ, if (x.snd = 0) then (g_zx.map x.fst, x.snd) else (g_wy.map x.fst, x.snd),
-
-  have g_simplicial : is_simplicial_map (Z ⋆ W) (X ⋆ Y) g, by sorry,--from
-  -- begin
-  --   unfold is_simplicial_map,
-  --   intros s s_in_ZW,
-  --   rw [simplicial_join_mem] at *,
-  --   simp only[simplex_disjoint_union] at *,
-
-  --   choose t t_in_Z u u_in_W s_eq_tu using s_in_ZW,
-  --   rw [s_eq_tu],
-  --   use (finset.image g_zx.map t),
-  --   split,
-  --   apply g_zx.is_simplicial,
-  --   assumption,
-
-  --   use (finset.image g_wy.map u),
-  --   split,
-  --   apply g_wy.is_simplicial,
-  --   assumption,
-
-  --   rw [finset.ext_iff],
-  --   intro x,
-  --   split,
-  --   { intro x_in_g,
-  --     rw [finset.image_union, finset.mem_union, finset.mem_image, finset.mem_image] at x_in_g,
-  --     rw [finset.mem_union],
-  --     cases x_in_g,
-      
-  --     left,
-  --     choose y y_in_t0 using x_in_g,
-  --     cases y_in_t0 with y_in_t0 gy_x,
-  --     rw [finset.mem_product] at y_in_t0,
-  --     cases y_in_t0 with y_in_t y0,
-  --     rw [finset.mem_product, finset.mem_image],
-  --     split,
-      
-  --     use y.fst,
-  --     split,
-  --     assumption,
-      
-  --     simp only[g] at gy_x,
-  --     revert gy_x,
-  --     split_ifs,
-      
-  --     intro gy_x,
-  --     rw [prod.eq_iff_fst_eq_snd_eq] at gy_x,
-  --     cases gy_x with gy_x_fst gy_x_snd,
-  --     assumption,
-      
-  --     rw [finset.mem_singleton] at y0,
-  --     contradiction,
-      
-  --     simp only[g] at gy_x,
-  --     revert gy_x,
-  --     split_ifs,
-      
-  --     intro gy_x,
-  --     rw [prod.eq_iff_fst_eq_snd_eq] at gy_x,
-  --     cases gy_x with gy_x_fst gy_x_snd,
-  --     rw [finset.mem_singleton, ←gy_x_snd],
-      
-  --     rw [finset.mem_singleton] at y0,
-  --     contradiction,
-      
-  --     right,
-  --     choose y y_in_u1 using x_in_g,
-  --     cases y_in_u1 with y_in_u1 gy_x,
-  --     rw [finset.mem_product] at y_in_u1,
-  --     cases y_in_u1 with y_in_u y1,
-  --     rw [finset.mem_product, finset.mem_image],
-  --     split,
-      
-  --     use y.fst,
-  --     split,
-  --     assumption,
-      
-  --     simp only[g] at gy_x,
-  --     revert gy_x,
-  --     split_ifs,
-      
-  --     rw [finset.mem_singleton] at y1,
-  --     finish,
-      
-  --     intro gy_x,
-  --     rw [prod.eq_iff_fst_eq_snd_eq] at gy_x,
-  --     cases gy_x with gy_x_fst gy_x_snd,
-  --     assumption,
-      
-  --     simp only[g] at gy_x,
-  --     revert gy_x,
-  --     split_ifs,
-      
-  --     rw [finset.mem_singleton] at y1,
-  --     finish,
-      
-  --     intro gy_x,
-  --     rw [prod.eq_iff_fst_eq_snd_eq] at gy_x,
-  --     cases gy_x with gy_x_fst gy_x_snd,
-  --     rw [finset.mem_singleton, ←gy_x_snd], },
-  --   { intro x_in_g_prod,
-  --     rw [finset.mem_union, finset.mem_product, finset.mem_product, finset.mem_image, finset.mem_image] at x_in_g_prod,
-  --     rw [finset.mem_image],
-  --     cases x_in_g_prod,
-      
-  --     cases x_in_g_prod with gzx_x x0,
-  --     choose y y_in_t gzx_x using gzx_x,
-  --     rw [finset.mem_singleton] at x0,
-      
-  --     use (y, 0),
-  --     split,
-
-  --     rw [finset.mem_union],
-  --     left,
-  --     rw [finset.mem_product],
-  --     split,
-  --     assumption,
-  --     simp,
-      
-  --     simp only[g],
-  --     split_ifs,
-      
-  --     rw [prod.eq_iff_fst_eq_snd_eq],
-  --     split,
-  --     assumption,
-  --     rw [x0],
-      
-  --     rw [prod.eq_iff_fst_eq_snd_eq],
-  --     split,
-  --     assumption,
-  --     rw [x0],
-      
-  --     cases x_in_g_prod with gzx_x x1,
-  --     choose y y_in_u gzx_x using gzx_x,
-  --     rw [finset.mem_singleton] at x1,
-      
-  --     use (y, 1),
-  --     split,
-      
-  --     rw [finset.mem_union],
-  --     right,
-  --     rw [finset.mem_product],
-  --     split,
-  --     assumption,
-  --     simp,
-      
-  --     simp only[g],
-  --     split_ifs,
-      
-  --     finish,
-      
-  --     rw [prod.eq_iff_fst_eq_snd_eq],
-  --     split,
-  --     assumption,
-  --     rw [x1], }
-  -- end,
+    simplicial_map.mk
+      (simplicial_join_iso_map f_xz.map f_yw.map)
+      (simplicial_join_iso_simplicial X Y Z W f_xz f_yw),
 
   let gs : simplicial_map (Z ⋆ W) (X ⋆ Y) :=
-    simplicial_map.mk g g_simplicial,
+    simplicial_map.mk
+      (simplicial_join_iso_map g_zx.map g_wy.map)
+      (simplicial_join_iso_simplicial Z W X Y g_zx g_wy),
 
   use fs,
   use gs,
   simp only[simplicial_map.map],
 
-  -- TODO: Fix.
   split; rw [function.funext_iff],
   { intro x,
-    simp only[id, function.comp, f, g],
+    simp only[id, function.comp, simplicial_join_iso_map],
     simp at *,
     split_ifs;
     rw [prod.eq_iff_fst_eq_snd_eq],
@@ -1949,7 +2361,7 @@ lemma simplicial_join_iso
     right,
     split; assumption, },
   { intro x,
-    simp only[id, function.comp, f, g],
+    simp only[id, function.comp, simplicial_join_iso_map],
     simp at *,
     split_ifs;
     rw [prod.eq_iff_fst_eq_snd_eq],
@@ -2013,40 +2425,1180 @@ lemma simplicial_join_iso_right
   assumption,
 end
 
+def simplicial_join_assoc_forward_aux
+    (X Y Z : simplicial_complex α)
+    (ψ : simplicial_coe (Y ⋆ Z) α)
+  : α × ℕ → α × ℕ
+:= λ x : α × ℕ, if (x.snd = 0) then x else (ψ.coe (x.fst, 0), x.snd)
+
+def simplicial_join_assoc_forward_map
+    (X Y Z : simplicial_complex α)
+    (φ : simplicial_coe (X ⋆ Y) α)
+    (ψ : simplicial_coe (Y ⋆ Z) α)
+    (f : simplicial_map (φ[X ⋆ Y]) (X ⋆ Y))
+  : α × ℕ → α × ℕ
+:= λ x : α × ℕ, if (x.snd = 0)
+    then ((simplicial_join_assoc_forward_aux X Y Z ψ) (f.map x.fst))
+    else (ψ.coe x, x.snd)
+
+-- set_option profiler true
+
+lemma simplicial_join_assoc_forward_simplicial_left
+    (X Y Z : simplicial_complex α)
+    (φ : simplicial_coe (X ⋆ Y) α)
+    (ψ : simplicial_coe (Y ⋆ Z) α)
+    (f : simplicial_map (φ[X ⋆ Y]) (X ⋆ Y))
+    (f_inv : is_inverse_simplicial_iso φ.simplicial_map f)
+    (a b t : finset α)
+    (a_in_X : a ∈ X.simplices)
+    (b_in_Y : b ∈ Y.simplices)
+    (t_in_Z : t ∈ Z.simplices)
+  : finset.image
+      (simplicial_join_assoc_forward_map X Y Z φ ψ f)
+      (finset.image φ.coe (a ⊔ₛ b) ⊔ₛ t)
+    ⊆ a ⊔ₛ finset.image ψ.coe (b ⊔ₛ t)
+:= begin
+  simp only [simplicial_join_assoc_forward_map, finset.subset_iff],
+  intros x x_in_img,
+  rw [finset.mem_image] at x_in_img,
+  choose y y_in_u img_y_x using x_in_img,
+
+  unfold is_inverse_simplicial_iso at f_inv,
+  simp only [set.restrict_eq_restrict_iff, set.eq_on, simplicial_map.comp, function.comp_app, id.def] at f_inv,
+  choose fφ_id φf_id using f_inv,
+  
+  simp only [simplex_disjoint_union, finset.mem_union, finset.mem_image, finset.mem_product, finset.mem_singleton],
+  revert img_y_x,
+  split_ifs,
+  
+  simp only [simplicial_join_assoc_forward_aux],
+  have y_rw : y = (y.fst, 0), from
+  begin
+    simp only [prod.ext_iff],
+    split, refl, assumption,
+  end,
+  rw [y_rw, simplex_disjoint_mem_left, finset.mem_image] at y_in_u,
+  choose z z_in_ab coe_z_y using y_in_u,
+
+  have z_in_join : z ∈ vertices (X ⋆ Y), from
+  begin
+    rw [vertex_iff_in_simplex],
+    use (a ⊔ₛ b), split,
+    rw [simplicial_join_mem],
+    use a, split, assumption,
+    use b, split, assumption,
+    refl,
+    assumption,
+  end,
+  specialize fφ_id z_in_join,
+  have coe_rw : φ.simplicial_map.map = φ.coe, by refl,
+  rw [coe_rw] at fφ_id,
+
+  split_ifs,
+  
+  intro fy_x,
+  left,
+  rw [←coe_z_y, fφ_id] at fy_x h_1,
+  subst fy_x,
+  
+  rw [simplex_disjoint_mem] at z_in_ab,
+  cases z_in_ab with z_in_a contra,
+  assumption,
+  choose z_in_b contra using contra,
+  have H : z.snd ≠ 0, by omega,
+  contradiction,
+  
+  intro ψfy_x,
+  right,
+  rw [←coe_z_y, fφ_id] at ψfy_x h_1,
+  subst ψfy_x,
+  simp only [prod.fst, prod.snd],
+  
+  rw [simplex_disjoint_mem] at z_in_ab,
+  cases z_in_ab with contra z_in_b,
+  choose z_in_a contra using contra,
+  contradiction,
+
+  choose z_in_b z_one using z_in_b,
+  split,
+  
+  use (z.fst, 0), split, left,
+  simp only [prod.fst, prod.snd],
+  split, assumption, refl,
+  
+  apply congr_arg, refl,
+  assumption,
+  
+  intro ψy_x,
+  right,
+  rw [simplex_disjoint_mem] at y_in_u,
+  cases y_in_u with contra y_in_t,
+  choose y_in_a contra using contra,
+  contradiction,
+  
+  choose y_in_t y_one using y_in_t,
+  simp only [prod.ext_iff] at ψy_x,
+  choose ψy_x x_one using ψy_x,
+  rw [y_one, @comm _ eq] at x_one,
+  split,
+  
+  use y, split,
+  right, split; assumption,
+  assumption,
+  assumption,
+end
+
+lemma simplicial_join_assoc_forward_simplicial_right
+    (X Y Z : simplicial_complex α)
+    (φ : simplicial_coe (X ⋆ Y) α)
+    (ψ : simplicial_coe (Y ⋆ Z) α)
+    (f : simplicial_map (φ[X ⋆ Y]) (X ⋆ Y))
+    (f_inv : is_inverse_simplicial_iso φ.simplicial_map f)
+    (a b t : finset α)
+    (a_in_X : a ∈ X.simplices)
+    (b_in_Y : b ∈ Y.simplices)
+    (t_in_Z : t ∈ Z.simplices)
+  : a ⊔ₛ finset.image ψ.coe (b ⊔ₛ t)
+    ⊆ finset.image
+        (simplicial_join_assoc_forward_map X Y Z φ ψ f)
+        (finset.image φ.coe (a ⊔ₛ b) ⊔ₛ t)
+:= begin
+  simp only [simplicial_join_assoc_forward_map, finset.subset_iff],
+  intros x x_in_join,
+
+  unfold is_inverse_simplicial_iso at f_inv,
+  simp only [set.restrict_eq_restrict_iff, set.eq_on, simplicial_map.comp, function.comp_app, id.def] at f_inv,
+  choose fφ_id φf_id using f_inv,
+  
+  simp only [simplex_disjoint_mem, finset.mem_image] at x_in_join,
+  simp only [finset.mem_image, simplicial_join_assoc_forward_aux],
+  cases x_in_join with x_in_a x_in_ψ,
+  
+  have x_in_XY : x ∈ vertices (X ⋆ Y), from
+  begin
+    rw [vertex_iff_in_simplex],
+    use (a ⊔ₛ b), split,
+    rw [simplicial_join_mem],
+    use a, split, assumption,
+    use b, split, assumption,
+    refl,
+    rw [simplex_disjoint_mem],
+    left, assumption,
+  end,
+  specialize fφ_id x_in_XY,
+  have coe_rw : φ.simplicial_map.map = φ.coe, by refl,
+  rw [coe_rw] at fφ_id,
+
+  use (φ.coe x, 0), split,
+  rw [simplex_disjoint_mem_left],
+  apply finset.mem_image_of_mem,
+  rw [simplex_disjoint_mem],
+  left, assumption,
+  
+  choose x_in_a x_zero using x_in_a,
+  simp only [fφ_id, x_zero, eq_self_iff_true, if_true],
+  
+  choose x_in_ψ x_one using x_in_ψ,
+  choose y y_in_bt ψy_x using x_in_ψ,
+  cases y_in_bt with y_in_b y_in_t,
+  
+  choose y_in_b y_zero using y_in_b,
+  use (φ.coe (y.fst, 1), 0), split,
+  rw [simplex_disjoint_mem_left],
+  apply finset.mem_image_of_mem,
+  rw [simplex_disjoint_mem],
+  right,
+  simp only [prod.fst, prod.snd],
+  split, assumption, refl,
+  
+  have y_in_XY : (y.fst, 1) ∈ vertices (X ⋆ Y), from
+  begin
+    rw [vertex_iff_in_simplex],
+    use (a ⊔ₛ b), split,
+    rw [simplicial_join_mem],
+    use a, split, assumption,
+    use b, split, assumption,
+    refl,
+    rw [simplex_disjoint_mem],
+    simp only [prod.fst, prod.snd],
+    right,
+    split, assumption, refl,
+  end,
+  specialize fφ_id y_in_XY,
+  have coe_rw : φ.simplicial_map.map = φ.coe, by refl,
+  rw [coe_rw] at fφ_id,
+  
+  simp only [fφ_id, y_zero, eq_self_iff_true, if_true, nat.one_ne_zero, if_false],
+  have y_rw : y = (y.fst, y.snd), from
+  begin
+    simp only [prod.ext_iff],
+    split; refl,
+  end,
+  rw [y_rw] at ψy_x,
+  rw [←y_zero, ←x_one, ψy_x],
+  simp only [prod.ext_iff],
+  split; refl,
+  
+  use y, split,
+  rw [simplex_disjoint_mem],
+  right, assumption,
+  
+  choose y_in_t y_one using y_in_t,
+  simp only [y_one, nat.one_ne_zero, if_false, prod.ext_iff],
+  rw [@comm _ eq] at x_one,
+  split, assumption, assumption,
+end
+
+lemma simplicial_join_assoc_forward_simplicial
+    (X Y Z : simplicial_complex α)
+    (φ : simplicial_coe (X ⋆ Y) α)
+    (ψ : simplicial_coe (Y ⋆ Z) α)
+    (f : simplicial_map (φ[X ⋆ Y]) (X ⋆ Y))
+    (f_inv : is_inverse_simplicial_iso φ.simplicial_map f)
+  : is_simplicial_map (φ[X ⋆ Y] ⋆ Z) (X ⋆ ψ[Y ⋆ Z]) (simplicial_join_assoc_forward_map X Y Z φ ψ f)
+:= begin
+  simp only [is_simplicial_map],
+  intros u u_in_join,
+  rw [simplicial_join_mem] at u_in_join ⊢,
+  choose s s_in_coe t t_in_z u_eq_st using u_in_join,
+  simp only [simplicial_image, simplicial_join, set.mem_set_of] at s_in_coe,
+  choose v v_in_join coe_v_s using s_in_coe,
+  choose a a_in_X b b_in_Y ab_eq_v using v_in_join,
+  subst ab_eq_v,
+  subst coe_v_s,
+  subst u_eq_st,
+  
+  use a, split, assumption,
+  use (finset.image ψ.coe (b ⊔ₛ t)), split,
+  simp only [simplicial_image, set.mem_set_of, simplicial_join_mem],
+  use (b ⊔ₛ t), split,
+  use b, split, assumption,
+  use t, split, assumption,
+  refl, refl,
+
+  simp only [simplicial_join_assoc_forward_map, finset.ext_iff],
+  intro x,
+  split,
+
+  apply simplicial_join_assoc_forward_simplicial_left;
+  assumption,
+
+  apply simplicial_join_assoc_forward_simplicial_right;
+  assumption,
+end
+
+def simplicial_join_assoc_inv_aux
+    (X Y Z : simplicial_complex α)
+    (φ : simplicial_coe (X ⋆ Y) α)
+  : α × ℕ → α × ℕ
+:= λ x : α × ℕ, if (x.snd = 0) then (φ.coe (x.fst, 1), 0) else x
+
+def simplicial_join_assoc_inv_map
+    (X Y Z : simplicial_complex α)
+    (φ : simplicial_coe (X ⋆ Y) α)
+    (ψ : simplicial_coe (Y ⋆ Z) α)
+    (g : simplicial_map (ψ[Y ⋆ Z]) (Y ⋆ Z))
+  : α × ℕ → α × ℕ
+:= λ x : α × ℕ, if (x.snd = 0)
+    then (φ.coe x, 0)
+    else ((simplicial_join_assoc_inv_aux X Y Z φ) (g.map x.fst))
+
+lemma simplicial_join_assoc_inv_simplicial_left
+    (X Y Z : simplicial_complex α)
+    (φ : simplicial_coe (X ⋆ Y) α)
+    (ψ : simplicial_coe (Y ⋆ Z) α)
+    (g : simplicial_map (ψ[Y ⋆ Z]) (Y ⋆ Z))
+    (g_inv : is_inverse_simplicial_iso ψ.simplicial_map g)
+    (s a b : finset α)
+    (s_in_X : s ∈ X.simplices)
+    (a_in_Y : a ∈ Y.simplices)
+    (b_in_Z : b ∈ Z.simplices)
+  : finset.image
+      (simplicial_join_assoc_inv_map X Y Z φ ψ g)
+      (s ⊔ₛ finset.image ψ.coe (a ⊔ₛ b))
+    ⊆ finset.image φ.coe (s ⊔ₛ a) ⊔ₛ b
+:= begin
+  simp only [simplicial_join_assoc_inv_map, finset.subset_iff],
+  intros x x_in_img,
+
+  unfold is_inverse_simplicial_iso at g_inv,
+  simp only [set.restrict_eq_restrict_iff, set.eq_on, simplicial_map.comp, function.comp_app, id.def] at g_inv,
+  choose gψ_id ψg_id using g_inv,
+
+  simp only [finset.mem_image, simplex_disjoint_mem, simplicial_join_assoc_inv_map] at x_in_img,
+  choose y y_in_join img_y_x using x_in_img,
+  
+  simp only [simplex_disjoint_union, finset.mem_union, finset.mem_image, finset.mem_product, finset.mem_singleton],
+  revert img_y_x,
+  split_ifs,
+  
+  cases y_in_join with y_in_s contra,
+  intro φy_x,
+  
+  left,
+  simp only [prod.ext_iff] at φy_x,
+  choose φy_x x_zero using φy_x,
+  rw [@comm _ eq] at x_zero,
+  use y, split,
+  left, assumption,
+  assumption,
+  assumption,
+  
+  choose y_in_coe contra using contra,
+  have H : y.snd ≠ 0, by omega,
+  contradiction,
+  
+  cases y_in_join with contra y_in_coe,
+  choose y_in_s contra using contra,
+  contradiction,
+  
+  choose y_in_coe y_one using y_in_coe,
+  choose z z_in_join ψz_y using y_in_coe,
+  simp only [simplicial_join_assoc_inv_aux],
+  intro img_y_x,
+  
+  have z_in_YZ : z ∈ vertices (Y ⋆ Z), from
+  begin
+    rw [vertex_iff_in_simplex],
+    use (a ⊔ₛ b), split,  
+    rw [simplicial_join_mem],
+    use a, split, assumption,
+    use b, split, assumption,
+    refl,
+    rw [simplex_disjoint_mem],
+    assumption,  
+  end,
+  specialize gψ_id z_in_YZ,
+  have coe_rw : ψ.simplicial_map.map = ψ.coe, by refl,
+  rw [coe_rw] at gψ_id,
+  
+  cases z_in_join with z_in_a z_in_b,
+  
+  left,
+  choose z_in_a z_zero using z_in_a,
+  simp only [←ψz_y, gψ_id, prod.ext_iff, z_zero, eq_self_iff_true, if_true] at img_y_x,
+  choose φz_x x_zero using img_y_x,
+  rw [@comm _ eq] at x_zero,
+  split,
+  use (z.fst, 1), split, right,
+  simp only [prod.fst, prod.snd],
+  split, assumption, refl,
+  assumption,
+  assumption,
+  
+  right,
+  choose z_in_b z_one using z_in_b,
+  simp only [←ψz_y, gψ_id, prod.ext_iff, z_one, nat.one_ne_zero, if_false] at img_y_x,
+  choose z_eq_x x_one using img_y_x,
+  rw [z_eq_x] at z_in_b,
+  rw [@comm _ eq] at x_one,
+  split; assumption,
+end
+
+lemma simplicial_join_assoc_inv_simplicial_right
+    (X Y Z : simplicial_complex α)
+    (φ : simplicial_coe (X ⋆ Y) α)
+    (ψ : simplicial_coe (Y ⋆ Z) α)
+    (g : simplicial_map (ψ[Y ⋆ Z]) (Y ⋆ Z))
+    (g_inv : is_inverse_simplicial_iso ψ.simplicial_map g)
+    (s a b : finset α)
+    (s_in_X : s ∈ X.simplices)
+    (a_in_Y : a ∈ Y.simplices)
+    (b_in_Z : b ∈ Z.simplices)
+  : finset.image φ.coe (s ⊔ₛ a) ⊔ₛ b
+    ⊆ finset.image
+        (simplicial_join_assoc_inv_map X Y Z φ ψ g)
+        (s ⊔ₛ finset.image ψ.coe (a ⊔ₛ b))
+:= begin
+  simp only [simplicial_join_assoc_inv_map, finset.subset_iff],
+  intros x x_in_join,
+
+  unfold is_inverse_simplicial_iso at g_inv,
+  simp only [set.restrict_eq_restrict_iff, set.eq_on, simplicial_map.comp, function.comp_app, id.def] at g_inv,
+  choose gψ_id ψg_id using g_inv,
+
+  simp only [simplex_disjoint_mem, finset.mem_image] at x_in_join,
+  simp only [finset.mem_image, simplicial_join_assoc_inv_map],
+  cases x_in_join with x_in_coe x_in_b,
+  
+  choose x_in_coe x_zero using x_in_coe,
+  choose y y_in_join φy_x using x_in_coe,
+  simp only [simplicial_join_assoc_inv_aux],
+  cases y_in_join with y_in_s y_in_a,
+  
+  use y, split,
+  rw [simplex_disjoint_mem],
+  left, assumption,
+  
+  choose y_in_s y_zero using y_in_s,
+  rw [@comm _ eq] at x_zero,
+  simp only [y_zero, eq_self_iff_true, if_true, prod.ext_iff],
+  split; assumption,
+  
+  choose y_in_a y_one using y_in_a,
+  use (ψ.coe (y.fst, 0), 1), split,
+  rw [simplex_disjoint_mem_right],
+  apply finset.mem_image_of_mem,
+  rw [simplex_disjoint_mem_left],
+  assumption,
+
+  have y_in_YZ : (y.fst, 0) ∈ vertices (Y ⋆ Z), from
+  begin
+    rw [vertex_iff_in_simplex],
+    use (a ⊔ₛ b), split,
+    rw [simplicial_join_mem],
+    use a, split, assumption,
+    use b, split, assumption,
+    refl,
+    rw [simplex_disjoint_mem_left],
+    assumption,
+  end,
+  specialize gψ_id y_in_YZ,
+  have coe_rw : ψ.simplicial_map.map = ψ.coe, by refl,
+  rw [coe_rw] at gψ_id,
+  
+  simp only [y_one, gψ_id, nat.one_ne_zero, if_false, eq_self_iff_true, if_true],
+  have y_rw : y = (y.fst, y.snd), from
+  begin
+    simp only [prod.ext_iff],
+    split; refl,
+  end,
+  rw [y_rw] at φy_x,
+  rw [←y_one, ←x_zero, φy_x],
+  simp only [prod.ext_iff],
+  split; refl,
+  
+  use (ψ.coe x, 1), split,
+  rw [simplex_disjoint_mem_right],
+  apply finset.mem_image_of_mem,
+  rw [simplex_disjoint_mem],
+  right, assumption,
+  
+  have x_in_YZ : x ∈ vertices (Y ⋆ Z), from
+  begin
+    rw [vertex_iff_in_simplex],
+    use (a ⊔ₛ b), split,
+    rw [simplicial_join_mem],
+    use a, split, assumption,
+    use b, split, assumption,
+    refl,
+    rw [simplex_disjoint_mem],
+    right, assumption,
+  end,
+  specialize gψ_id x_in_YZ,
+  have coe_rw : ψ.simplicial_map.map = ψ.coe, by refl,
+  rw [coe_rw] at gψ_id,
+  
+  choose x_in_b x_one using x_in_b,
+  simp only [simplicial_join_assoc_inv_aux],
+  simp only [prod.snd, x_one, gψ_id, nat.one_ne_zero, if_false],
+end
+
+lemma simplicial_join_assoc_inv_simplicial
+    (X Y Z : simplicial_complex α)
+    (φ : simplicial_coe (X ⋆ Y) α)
+    (ψ : simplicial_coe (Y ⋆ Z) α)
+    (g : simplicial_map (ψ[Y ⋆ Z]) (Y ⋆ Z))
+    (g_inv : is_inverse_simplicial_iso ψ.simplicial_map g)
+  : is_simplicial_map (X ⋆ ψ[Y ⋆ Z]) (φ[X ⋆ Y] ⋆ Z) (simplicial_join_assoc_inv_map X Y Z φ ψ g)
+:= begin
+  simp only [is_simplicial_map],
+  intros u u_in_join,
+  rw [simplicial_join_mem] at u_in_join ⊢,
+  choose s s_in_X t t_in_coe u_eq_st using u_in_join,
+  simp only [simplicial_image, simplicial_join, set.mem_set_of] at t_in_coe,
+  choose v v_in_join coe_v_s using t_in_coe,
+  choose a a_in_Y b b_in_Z ab_eq_v using v_in_join,
+  subst ab_eq_v,
+  subst coe_v_s,
+  subst u_eq_st,
+  
+  use (finset.image φ.coe (s ⊔ₛ a)), split,
+  simp only [simplicial_image, set.mem_set_of, simplicial_join_mem],
+  use (s ⊔ₛ a), split,
+  use s, split, assumption,
+  use a, split, assumption,
+  refl, refl,
+  use b, split, assumption,
+
+  simp only [simplicial_join_assoc_forward_map, finset.ext_iff],
+  intro x,
+  split,
+
+  apply simplicial_join_assoc_inv_simplicial_left;
+  assumption,
+
+  apply simplicial_join_assoc_inv_simplicial_right;
+  assumption,
+end
+
 lemma simplicial_join_assoc
+    [nonempty α]
     (X Y Z : simplicial_complex α)
     (φ : simplicial_coe (X ⋆ Y) α)
     (ψ : simplicial_coe (Y ⋆ Z) α)
   : φ[(X ⋆ Y)] ⋆ Z ≅ X ⋆ ψ[(Y ⋆ Z)]
-:= sorry
+:= begin
+  have φ_iso : is_simplicial_iso φ.simplicial_map, by apply coe_is_iso,
+  have ψ_iso : is_simplicial_iso ψ.simplicial_map, by apply coe_is_iso,
+
+  unfold is_simplicial_iso at φ_iso ψ_iso,
+  choose gXY gφ_inv using φ_iso,
+  choose gYZ gψ_inv using ψ_iso,
+
+  let f_assoc : simplicial_map (φ[X ⋆ Y] ⋆ Z) (X ⋆ ψ[Y ⋆ Z]) :=
+    simplicial_map.mk
+      (simplicial_join_assoc_forward_map X Y Z φ ψ gXY)
+      (simplicial_join_assoc_forward_simplicial X Y Z φ ψ gXY gφ_inv),
+
+  let g_assoc : simplicial_map (X ⋆ ψ[Y ⋆ Z]) (φ[X ⋆ Y] ⋆ Z) :=
+    simplicial_map.mk
+      (simplicial_join_assoc_inv_map X Y Z φ ψ gYZ)
+      (simplicial_join_assoc_inv_simplicial X Y Z φ ψ gYZ gψ_inv),
+
+  unfold is_inverse_simplicial_iso at gφ_inv gψ_inv,
+  simp only [set.restrict_eq_restrict_iff, set.eq_on, simplicial_map.comp, function.comp_app, id.def] at gφ_inv gψ_inv,
+  
+  have φ_rw : φ.simplicial_map.map = φ.coe, by refl,
+  have ψ_rw : ψ.simplicial_map.map = ψ.coe, by refl,
+  simp only [φ_rw] at gφ_inv,
+  simp only [ψ_rw] at gψ_inv,
+
+  choose gφ_id φg_id using gφ_inv,
+  choose gψ_id ψg_id using gψ_inv,
+
+  unfold is_simplicially_iso,
+  use f_assoc,
+
+  unfold is_simplicial_iso,
+  use g_assoc,
+
+  unfold is_inverse_simplicial_iso,
+  simp only [set.restrict_eq_restrict_iff, set.eq_on, simplicial_map.comp, function.comp_app, id.def],
+  simp only [simplicial_join_assoc_forward_map, simplicial_join_assoc_inv_map],
+  split,
+
+  { intros x x_in_join,
+    rw [vertex_iff_in_simplex] at x_in_join,
+    choose u u_in_join x_in_u using x_in_join,
+    simp only [simplicial_join_mem, simplicial_image, set.mem_set_of] at u_in_join,
+    choose s s_in_coe t t_in_Z u_eq_st using u_in_join,
+    choose v v_in_join coe_v_s using s_in_coe,
+    choose a a_in_X b b_in_Y v_eq_ab using v_in_join,
+    subst v_eq_ab,
+    subst coe_v_s,
+    subst u_eq_st,
+    
+    simp only [finset.mem_image, simplex_disjoint_mem] at x_in_u,
+    cases x_in_u with x_in_coe x_in_t,
+    
+    choose x_in_coe x_zero using x_in_coe,
+    choose y y_in_join φy_x using x_in_coe,
+    simp only [←φy_x, x_zero, eq_self_iff_true, if_true],
+    simp only [simplicial_join_assoc_forward_aux, simplicial_join_assoc_inv_aux],
+
+    have y_in_XY : y ∈ vertices (X ⋆ Y), from
+    begin
+      rw [vertex_iff_in_simplex],
+      use (a ⊔ₛ b), split,
+      rw [simplicial_join_mem],
+      use a, split, assumption,
+      use b, split, assumption,
+      refl,
+      rw [simplex_disjoint_mem],
+      assumption,
+    end,
+    specialize gφ_id y_in_XY,
+    simp only [gφ_id],
+    cases y_in_join with y_in_a y_in_b,
+    
+    choose y_in_a y_zero using y_in_a,
+    simp only [y_zero, eq_self_iff_true, if_true, prod.snd, prod.ext_iff],
+    rw [@comm _ eq] at x_zero,
+    split; assumption,
+    
+    choose y_in_b y_one using y_in_b,
+    have y_in_YZ : (y.fst, 0) ∈ vertices (Y ⋆ Z), from
+    begin
+      rw [simplicial_join_vertices_mem_left, vertex_iff_in_simplex],
+      use b, split; assumption,
+    end,
+    specialize gψ_id y_in_YZ,
+    simp only [gψ_id, y_one, eq_self_iff_true, if_true, nat.one_ne_zero, if_false, prod.snd, prod.ext_iff],
+    have y_rw : y = (y.fst, y.snd), from
+    begin
+      simp only [prod.ext_iff],
+      split; refl,
+    end,
+    rw [@comm _ eq] at x_zero,
+    rw [←y_one, ←y_rw],
+    split; assumption,
+    
+    have x_in_YZ : x ∈ vertices (Y ⋆ Z), from
+    begin
+      rw [vertex_iff_in_simplex],
+      use (b ⊔ₛ t), split,
+      rw [simplicial_join_mem],
+      use b, split, assumption,
+      use t, split, assumption,
+      refl,
+      rw [simplex_disjoint_mem],
+      right, assumption,
+    end,
+    choose x_in_t x_one using x_in_t,
+    specialize gψ_id x_in_YZ,
+    simp only [simplicial_join_assoc_inv_aux],
+    simp only [gψ_id, x_one, nat.one_ne_zero, if_false], },
+
+  { intros x x_in_join,
+    rw [vertex_iff_in_simplex] at x_in_join,
+    choose u u_in_join x_in_u using x_in_join,
+    simp only [simplicial_join_mem, simplicial_image, set.mem_set_of] at u_in_join,
+    choose s s_in_X t t_in_coe u_eq_st using u_in_join,
+    choose v v_in_join coe_v_t using t_in_coe,
+    choose a a_in_X b b_in_Y v_eq_ab using v_in_join,
+    subst v_eq_ab,
+    subst coe_v_t,
+    subst u_eq_st,
+    
+    simp only [finset.mem_image, simplex_disjoint_mem] at x_in_u,
+    cases x_in_u with x_in_s x_in_coe,
+    
+    have x_in_XY : x ∈ vertices (X ⋆ Y), from
+    begin
+      rw [vertex_iff_in_simplex],
+      use (s ⊔ₛ a), split,
+      rw [simplicial_join_mem],
+      use s, split, assumption,
+      use a, split, assumption,
+      refl,
+      rw [simplex_disjoint_mem],
+      left, assumption,
+    end,
+    choose x_in_s x_one using x_in_s,
+    specialize gφ_id x_in_XY,
+    simp only [simplicial_join_assoc_forward_aux],
+    simp only [gφ_id, x_one, eq_self_iff_true, if_true],
+    
+    choose x_in_coe x_one using x_in_coe,
+    choose y y_in_join ψy_x using x_in_coe,
+    cases y_in_join with y_in_a y_in_b,
+    
+    have y_in_YZ : y ∈ vertices (Y ⋆ Z), from
+    begin
+      rw [vertex_iff_in_simplex],
+      use (a ⊔ₛ b), split,
+      rw [simplicial_join_mem],
+      use a, split, assumption,
+      use b, split, assumption,
+      refl,
+      rw [simplex_disjoint_mem],
+      left, assumption,
+    end,
+    choose y_in_a y_zero using y_in_a,
+    specialize gψ_id y_in_YZ,
+
+    have y_in_XY : (y.fst, 1) ∈ vertices (X ⋆ Y), from
+    begin
+      rw [simplicial_join_vertices_mem_right, vertex_iff_in_simplex],
+      use a, split; assumption,
+    end,
+    specialize gφ_id y_in_XY,
+
+    simp only [simplicial_join_assoc_forward_aux, simplicial_join_assoc_inv_aux],
+    simp only [←ψy_x, gψ_id, gφ_id, y_zero, x_one, eq_self_iff_true, if_true, nat.one_ne_zero, if_false, prod.snd],
+    have y_rw : y = (y.fst, y.snd), from
+    begin
+      simp only [prod.ext_iff],
+      split; refl,
+    end,
+    rw [←y_zero, ←y_rw],
+    rw [@comm _ eq] at x_one,
+    simp only [prod.ext_iff],
+    split; assumption,
+    
+    have y_in_YZ : y ∈ vertices (Y ⋆ Z), from
+    begin
+      rw [vertex_iff_in_simplex],
+      use (a ⊔ₛ b), split,
+      rw [simplicial_join_mem],
+      use a, split, assumption,
+      use b, split, assumption,
+      refl,
+      rw [simplex_disjoint_mem],
+      right, assumption,
+    end,
+    choose y_in_b y_one using y_in_b,
+    specialize gψ_id y_in_YZ,
+    
+    simp only [simplicial_join_assoc_forward_aux, simplicial_join_assoc_inv_aux],
+    simp only [←ψy_x, gψ_id, y_one, x_one, nat.one_ne_zero, if_false, prod.ext_iff],
+    split; refl, },
+end
+
+def simplicial_join_comm_map
+  : α × ℕ → α × ℕ
+:= λ x : α × ℕ, if (x.snd = 0) then (x.fst, 1) else (x.fst, 0)
+
+lemma simplicial_join_comm_simplicial
+    (X Y : simplicial_complex α)
+  : is_simplicial_map (X ⋆ Y) (Y ⋆ X) (simplicial_join_comm_map)
+:= begin
+  simp only [is_simplicial_map, simplicial_join, set.mem_set_of],
+  intros u u_in_XY,
+  choose s s_in_X t t_in_Y st_eq_u using u_in_XY,
+
+  use t, split, assumption,
+  use s, split, assumption,
+
+  simp only [simplicial_join_comm_map, finset.ext_iff],
+  intro x, split,
+
+  { intro x_in_ts,
+    rw [simplex_disjoint_mem] at x_in_ts,
+    rw [finset.mem_image],
+    cases x_in_ts with x_in_t x_in_s,
+    
+    choose x_in_t x_zero using x_in_t,
+    use (x.fst, 1), split,
+    rw [←st_eq_u, simplex_disjoint_mem_right],
+    assumption,
+    
+    simp only [nat.one_ne_zero, if_false],
+    simp only [←x_zero, prod.ext_iff],
+    split; refl,
+    
+    choose x_in_s x_one using x_in_s,
+    use (x.fst, 0), split,
+    rw [←st_eq_u, simplex_disjoint_mem_left],
+    assumption,
+    
+    simp only [eq_self_iff_true, if_true],
+    simp only [←x_one, prod.ext_iff],
+    split; refl, },
+
+  { intro x_in_img,
+    rw [finset.mem_image] at x_in_img,
+    rw [simplex_disjoint_mem],
+    choose y y_in_u fy_eq_x using x_in_img,
+    revert fy_eq_x,
+    split_ifs,
+    
+    intro y_one_x,
+    simp only [prod.ext_iff, prod.fst, prod.snd] at y_one_x,
+    choose y_eq_x x_one using y_one_x,
+    rw [@comm _ eq] at x_one,
+    rw [←st_eq_u, simplex_disjoint_mem] at y_in_u,
+    cases y_in_u with y_in_s contra,
+    
+    choose y_in_s y_zero using y_in_s,
+    rw [y_eq_x] at y_in_s,
+    right, split; assumption,
+    
+    choose y_in_t contra using contra,
+    have H : y.snd ≠ 0, by omega,
+    contradiction,
+    
+    intro y_zero_x,
+    simp only [prod.ext_iff, prod.fst, prod.snd] at y_zero_x,
+    choose y_eq_x x_zero using y_zero_x,
+    rw [@comm _ eq] at x_zero,
+    rw [←st_eq_u, simplex_disjoint_mem] at y_in_u,
+    cases y_in_u with contra y_in_t,
+    
+    choose y_in_s contra using contra,
+    contradiction,
+    
+    choose y_in_t y_one using y_in_t,
+    rw [y_eq_x] at y_in_t,
+    left, split; assumption, },
+end
 
 lemma simplicial_join_comm
     (X Y : simplicial_complex α)
   : X ⋆ Y ≅ Y ⋆ X
-:= sorry
+:= begin
+  let f : simplicial_map (X ⋆ Y) (Y ⋆ X) :=
+    simplicial_map.mk
+      (simplicial_join_comm_map)
+      (simplicial_join_comm_simplicial X Y),
+
+  let g : simplicial_map (Y ⋆ X) (X ⋆ Y) :=
+    simplicial_map.mk
+      (simplicial_join_comm_map)
+      (simplicial_join_comm_simplicial Y X),
+
+  unfold is_simplicially_iso,
+  use f,
+  
+  unfold is_simplicial_iso,
+  use g,
+
+  unfold is_inverse_simplicial_iso,
+  split;
+
+  { simp only [set.restrict_eq_restrict_iff, set.eq_on],
+    intros x x_in_XY,
+    rw [simplicial_join_mem_vertices] at x_in_XY,
+    simp only [f, g, simplicial_map.comp, simplicial_join_comm_map, id.def, function.comp_app],
+    cases x_in_XY with x_in_X x_in_Y,
+    
+    choose x_in_X x_zero using x_in_X,
+    simp only [x_zero, eq_self_iff_true, if_true, nat.one_ne_zero, if_false],
+    simp only [←x_zero, prod.ext_iff, prod.fst, prod.snd],
+    split; refl,
+    
+    choose x_in_Y x_one using x_in_Y,
+    simp only [x_one, eq_self_iff_true, if_true, nat.one_ne_zero, if_false],
+    simp only [←x_one, prod.ext_iff, prod.fst, prod.snd],
+    split; refl, },
+end
 
 -- Make sense of natural projections, inclusions, etc.
+def simplicial_join_id_forward_map
+  : α × ℕ → α
+:= λ x : α × ℕ, x.fst
+
+lemma simplicial_join_id_left_forward_simplicial
+    (X : simplicial_complex α)
+  : is_simplicial_map (X ⋆ empty_sc) X simplicial_join_id_forward_map
+:= begin
+  simp only [is_simplicial_map, simplicial_join_id_forward_map, empty_sc],
+  intros u u_in_X_empty,
+  rw [simplicial_join_mem] at u_in_X_empty,
+  choose s s_in_X t t_in_empty st_eq_u using u_in_X_empty,
+
+  rw [set.mem_singleton_iff] at t_in_empty,
+  simp only [t_in_empty, simplex_disjoint_union, finset.empty_product, finset.union_empty] at st_eq_u,
+  simp only [st_eq_u],
+  
+  have s_img : finset.image prod.fst (s ×ˢ {0}) = s, from
+  begin
+    simp only [finset.ext_iff, finset.mem_image],
+    intro x,
+    split,
+
+    intro x_in_img,
+    choose y y_in_prod proj_y_x using x_in_img,
+    rw [finset.mem_product] at y_in_prod,
+    choose y_in_s y_zero using y_in_prod,
+    rw [←proj_y_x],
+    assumption,
+
+    intro x_in_s,
+    use (x, 0), split,
+    simp only [finset.mem_product, prod.fst, prod.snd],
+    split,
+    assumption,
+    apply finset.mem_singleton_self,
+
+    simp only [prod.fst],
+  end,
+
+  rw [s_img],
+  assumption,
+end
+
+def simplicial_join_id_left_inverse_map
+  : α → α × ℕ
+:= λ x : α, (x, 0)
+
+lemma simplicial_join_id_left_inverse_simplicial
+    (X : simplicial_complex α)
+  : is_simplicial_map X (X ⋆ empty_sc) (simplicial_join_id_left_inverse_map)
+:= begin
+  simp only [is_simplicial_map],
+  intros u u_in_X,
+  simp only [simplicial_join, empty_sc, set.mem_set_of],
+
+  use u, split, assumption,
+  use ∅, split, apply simplicial_complex_empty_simplex,
+
+  have u_img : finset.image simplicial_join_id_left_inverse_map u = u ×ˢ {0}, from
+  begin
+    simp only [simplicial_join_id_left_inverse_map, finset.ext_iff, finset.mem_image, finset.mem_product],
+    intro x,
+    split,
+
+    intro x_in_img,
+    choose y y_in_u inj_y_x using x_in_img,
+    simp only [prod.ext_iff, prod.fst, prod.snd] at inj_y_x,
+    choose y_eq_x x_zero using inj_y_x,
+    rw [@comm _ eq, ←finset.mem_singleton] at x_zero,
+    rw [y_eq_x] at y_in_u,
+    split; assumption,
+
+    intro x_in_prod,
+    choose x_in_u x_zero using x_in_prod,
+    rw [finset.mem_singleton, @comm _ eq] at x_zero,
+    use x.fst, split, assumption,
+    simp only [prod.ext_iff, prod.fst, prod.snd],
+    split, refl, assumption,
+  end,
+
+  simp only [u_img, simplex_disjoint_union, finset.empty_product, finset.union_empty],
+end
+
 lemma simplicial_join_id_left
     (X : simplicial_complex α)
   : X ⋆ empty_sc ≅ X
-:= sorry
+:= begin
+  let f : simplicial_map (X ⋆ empty_sc) X :=
+    simplicial_map.mk
+      (simplicial_join_id_forward_map)
+      (simplicial_join_id_left_forward_simplicial X),
+
+  let g : simplicial_map X (X ⋆ empty_sc) :=
+    simplicial_map.mk
+      (simplicial_join_id_left_inverse_map)
+      (simplicial_join_id_left_inverse_simplicial X),
+
+  unfold is_simplicially_iso,
+  use f,
+
+  unfold is_simplicial_iso,
+  use g,
+
+  unfold is_inverse_simplicial_iso,
+  split,
+
+  { simp only [set.restrict_eq_restrict_iff, set.eq_on],
+    intros x x_in_X_empty,
+    rw [simplicial_join_mem_vertices] at x_in_X_empty,
+    simp only [f, g, simplicial_join_id_forward_map, simplicial_join_id_left_inverse_map],
+    simp only [simplicial_map.comp, function.comp_app, id.def, prod.ext_iff, prod.fst, prod.snd],
+    cases x_in_X_empty with x_in_X contra,
+    
+    choose x_in_X x_zero using x_in_X,
+    rw [@comm _ eq] at x_zero,
+    split,
+    refl,
+    assumption,
+    
+    choose contra x_one using contra,
+    rw [empty_sc_vertices] at contra,
+    have H : x.fst ∉ ∅, by apply set.not_mem_empty x.fst,
+    contradiction, },
+
+  { simp only [set.restrict_eq_restrict_iff, set.eq_on],
+    intros x x_in_X,
+    simp only [f, g, simplicial_join_id_forward_map, simplicial_join_id_left_inverse_map],
+    simp only [simplicial_map.comp, function.comp_app, id.def], },
+end
+
+lemma simplicial_join_id_right_forward_simplicial
+    (X : simplicial_complex α)
+  : is_simplicial_map (empty_sc ⋆ X) X simplicial_join_id_forward_map
+:= begin
+  simp only [is_simplicial_map, simplicial_join_id_forward_map, empty_sc],
+  intros u u_in_empty_X,
+  rw [simplicial_join_mem] at u_in_empty_X,
+  choose s s_in_empty t t_in_X st_eq_u using u_in_empty_X,
+
+  rw [set.mem_singleton_iff] at s_in_empty,
+  simp only [s_in_empty, simplex_disjoint_union, finset.empty_product, finset.empty_union] at st_eq_u,
+  simp only [st_eq_u],
+  
+  have t_img : finset.image prod.fst (t ×ˢ {1}) = t, from
+  begin
+    simp only [finset.ext_iff, finset.mem_image],
+    intro x,
+    split,
+
+    intro x_in_img,
+    choose y y_in_prod proj_y_x using x_in_img,
+    rw [finset.mem_product] at y_in_prod,
+    choose y_in_s y_zero using y_in_prod,
+    rw [←proj_y_x],
+    assumption,
+
+    intro x_in_t,
+    use (x, 1), split,
+    simp only [finset.mem_product, prod.fst, prod.snd],
+    split,
+    assumption,
+    apply finset.mem_singleton_self,
+
+    simp only [prod.fst],
+  end,
+
+  rw [t_img],
+  assumption,
+end
+
+def simplicial_join_id_right_inverse_map
+  : α → α × ℕ
+:= λ x : α, (x, 1)
+
+lemma simplicial_join_id_right_inverse_simplicial
+    (X : simplicial_complex α)
+  : is_simplicial_map X (empty_sc ⋆ X) simplicial_join_id_right_inverse_map
+:= begin
+  simp only [is_simplicial_map],
+  intros u u_in_X,
+  simp only [simplicial_join, empty_sc, set.mem_set_of],
+
+  use ∅, split, apply simplicial_complex_empty_simplex,
+  use u, split, assumption,
+
+  have u_img : finset.image simplicial_join_id_right_inverse_map u = u ×ˢ {1}, from
+  begin
+    simp only [simplicial_join_id_right_inverse_map, finset.ext_iff, finset.mem_image, finset.mem_product],
+    intro x,
+    split,
+
+    intro x_in_img,
+    choose y y_in_u inj_y_x using x_in_img,
+    simp only [prod.ext_iff, prod.fst, prod.snd] at inj_y_x,
+    choose y_eq_x x_zero using inj_y_x,
+    rw [@comm _ eq, ←finset.mem_singleton] at x_zero,
+    rw [y_eq_x] at y_in_u,
+    split; assumption,
+
+    intro x_in_prod,
+    choose x_in_u x_zero using x_in_prod,
+    rw [finset.mem_singleton, @comm _ eq] at x_zero,
+    use x.fst, split, assumption,
+    simp only [prod.ext_iff, prod.fst, prod.snd],
+    split, refl, assumption,
+  end,
+
+  simp only [u_img, simplex_disjoint_union, finset.empty_product, finset.empty_union],
+end
 
 lemma simplicial_join_id_right
     (X : simplicial_complex α)
   : empty_sc ⋆ X ≅ X
-:= sorry
+:= begin
+  let f : simplicial_map (empty_sc ⋆ X) X :=
+    simplicial_map.mk
+      (simplicial_join_id_forward_map)
+      (simplicial_join_id_right_forward_simplicial X),
+
+  let g : simplicial_map X (empty_sc ⋆ X) :=
+    simplicial_map.mk
+      (simplicial_join_id_right_inverse_map)
+      (simplicial_join_id_right_inverse_simplicial X),
+
+  unfold is_simplicially_iso,
+  use f,
+
+  unfold is_simplicial_iso,
+  use g,
+
+  unfold is_inverse_simplicial_iso,
+  split,
+
+  { simp only [set.restrict_eq_restrict_iff, set.eq_on],
+    intros x x_in_empty_X,
+    rw [simplicial_join_mem_vertices] at x_in_empty_X,
+    simp only [f, g, simplicial_join_id_forward_map, simplicial_join_id_right_inverse_map],
+    simp only [simplicial_map.comp, function.comp_app, id.def, prod.ext_iff, prod.fst, prod.snd],
+    cases x_in_empty_X with contra x_in_X,
+
+    choose contra x_one using contra,
+    rw [empty_sc_vertices] at contra,
+    have H : x.fst ∉ ∅, by apply set.not_mem_empty x.fst,
+    contradiction,
+    
+    choose x_in_X x_zero using x_in_X,
+    rw [@comm _ eq] at x_zero,
+    split,
+    refl,
+    assumption, },
+
+  { simp only [set.restrict_eq_restrict_iff, set.eq_on],
+    intros x x_in_X,
+    simp only [f, g, simplicial_join_id_forward_map, simplicial_join_id_right_inverse_map],
+    simp only [simplicial_map.comp, function.comp_app, id.def], },
+end
 
 lemma simplicial_join_natural_incl_left
     (X Y : simplicial_complex α)
     (t : finset α)
   : t ∈ Y.simplices ↔ X ⋆ simplex t ⊆ X ⋆ Y
-:= sorry
+:= begin
+  simp only [simplicial_join, is_subcomplex, set.subset_def, set.mem_set_of],
+  split,
+
+  -- t ∈ Y case.
+  intros t_in_Y u u_in_join,
+  choose s s_in_X v v_in_Y sv_eq_u using u_in_join,
+
+  use s, split, assumption,
+  use v, split,
+  apply simplex_if_in_subcomplex (simplex t),
+  assumption,
+  rw [←simplex_iff_subcomplex_mem],
+  assumption,
+  assumption,
+
+  -- X ⋆ t ⊆ X ⋆ Y case.
+  intros X_sub_Y,
+  specialize X_sub_Y (∅ ⊔ₛ t),
+
+  have X_mem : ∃ (s : finset α) (H : s ∈ X.simplices) (v : finset α) (H : v ∈ (simplex t).simplices),
+      s ⊔ₛ v = ∅ ⊔ₛ t, from
+  begin
+    use ∅, split, apply simplicial_complex_empty_simplex,
+    use t, split,
+    simp only [simplex, finset.mem_coe],
+    apply finset.mem_powerset_self,
+    refl,
+  end,
+  specialize X_sub_Y X_mem,
+
+  choose s s_in_X v v_in_Y sv_eq_t using X_sub_Y,
+  rw [simplex_disjoint_eq_unique] at sv_eq_t,
+  choose s_empty v_eq_t using sv_eq_t,
+  subst v_eq_t,
+  assumption,
+end
 
 lemma simplicial_join_natural_incl_right
     (X Y : simplicial_complex α)
     (s : finset α)
   : s ∈ X.simplices ↔ simplex s ⋆ Y ⊆ X ⋆ Y
-:= sorry
+:= begin
+  simp only [simplicial_join, is_subcomplex, set.subset_def, set.mem_set_of],
+  split,
+
+  -- s ∈ X case.
+  intros s_in_X u u_in_join,
+  choose t t_in_X v v_in_Y tv_eq_u using u_in_join,
+
+  use t, split,
+  apply simplex_if_in_subcomplex (simplex s),
+  assumption,
+  rw [←simplex_iff_subcomplex_mem],
+  assumption,
+  use v, split,
+  assumption,
+  assumption,
+
+  -- X ⋆ t ⊆ X ⋆ Y case.
+  intros X_sub_Y,
+  specialize X_sub_Y (s ⊔ₛ ∅),
+
+  have Y_mem : ∃ (t : finset α) (H : t ∈ (simplex s).simplices) (v : finset α) (H : v ∈ Y.simplices),
+      t ⊔ₛ v = s ⊔ₛ ∅, from
+  begin
+    use s, split,
+    simp only [simplex, finset.mem_coe],
+    apply finset.mem_powerset_self,
+
+    use ∅, split, apply simplicial_complex_empty_simplex,
+
+    refl,
+  end,
+  specialize X_sub_Y Y_mem,
+
+  choose t t_in_X v v_in_Y tv_eq_s using X_sub_Y,
+  rw [simplex_disjoint_eq_unique] at tv_eq_s,
+  choose s_eq_t v_empty using tv_eq_s,
+  subst s_eq_t,
+  assumption,
+end
 
 lemma simplicial_join_subcomplex
     (X Y Z W : simplicial_complex α)
@@ -2071,13 +3623,95 @@ end
 
 lemma simplicial_join_distr_union_left
     (X Y Z : simplicial_complex α)
+  : (X ⋆ (Y ∪ Z)).simplices = ((X ⋆ Y) ∪ (X ⋆ Z)).simplices
+:= begin
+  simp only [simplicial_join, simplicial_union, set.ext_iff, set.mem_union, set.mem_set_of],
+  intro u,
+  split,
+
+  { intro u_in_join,
+    choose s s_in_X t t_in_YZ st_eq_u using u_in_join,
+    cases t_in_YZ with t_in_Y t_in_Z,
+    
+    left,
+    use s, split, assumption,
+    use t, split, assumption,
+    assumption,
+    
+    right,
+    use s, split, assumption,
+    use t, split, assumption,
+    assumption, },
+
+  { intro u_in_union,
+    cases u_in_union with u_in_XY u_in_XZ,
+    
+    choose s s_in_X t t_in_Y st_eq_u using u_in_XY,
+    use s, split, assumption,
+    use t, split,
+    left, assumption,
+    assumption,
+    
+    choose s s_in_X t t_in_Z st_eq_u using u_in_XZ,
+    use s, split, assumption,
+    use t, split,
+    right, assumption,
+    assumption, },
+end
+
+lemma simplicial_join_distr_union_left_iso
+    (X Y Z : simplicial_complex α)
   : X ⋆ (Y ∪ Z) ≅ (X ⋆ Y) ∪ (X ⋆ Z)
-:= sorry
+:= begin
+  apply simplicial_iso_preserves_equiv,
+  apply simplicial_join_distr_union_left,
+end
 
 lemma simplicial_join_distr_union_right
     (X Y Z : simplicial_complex α)
+  : ((Y ∪ Z) ⋆ X).simplices = ((Y ⋆ X) ∪ (Z ⋆ X)).simplices
+:= begin
+  simp only [simplicial_join, simplicial_union, set.ext_iff, set.mem_union, set.mem_set_of],
+  intro u,
+  split,
+
+  { intro u_in_join,
+    choose s s_in_YZ t t_in_X st_eq_u using u_in_join,
+    cases s_in_YZ with s_in_Y s_in_Z,
+    
+    left,
+    use s, split, assumption,
+    use t, split, assumption,
+    assumption,
+    
+    right,
+    use s, split, assumption,
+    use t, split, assumption,
+    assumption, },
+
+  { intro u_in_union,
+    cases u_in_union with u_in_XY u_in_XZ,
+    
+    choose s s_in_X t t_in_Y st_eq_u using u_in_XY,
+    use s, split,
+    left, assumption,
+    use t, split, assumption,
+    assumption,
+    
+    choose s s_in_X t t_in_Z st_eq_u using u_in_XZ,
+    use s, split,
+    right, assumption,
+    use t, split, assumption,
+    assumption, },
+end
+
+lemma simplicial_join_distr_union_right_iso
+    (X Y Z : simplicial_complex α)
   : (Y ∪ Z) ⋆ X ≅ (Y ⋆ X) ∪ (Z ⋆ X)
-:= sorry
+:= begin
+  apply simplicial_iso_preserves_equiv,
+  apply simplicial_join_distr_union_right,
+end
 
 -- Lemma 2.1, p.5
 lemma dim_of_join
@@ -2085,10 +3719,60 @@ lemma dim_of_join
   : dim_of_complex (X ⋆ Y) = (dim_of_complex X) + (dim_of_complex Y) + 1
 := begin
   intros,
+  set k := dim_of_complex (X ⋆ Y),
   set n := dim_of_complex X,
   set m := dim_of_complex Y,
-  unfold dim_of_complex,
-  sorry,
+
+  rw [le_antisymm_iff],
+  split,
+
+  { have k_dim : k ∈ finset.image dim (X ⋆ Y).simplices.to_finset, by apply finset.max'_mem,
+    simp only [finset.mem_image, set.mem_to_finset] at k_dim,
+    choose u u_in_XY dim_u_k using k_dim,
+    rw [simplicial_join_mem] at u_in_XY,
+    choose s s_in_X t t_in_Y u_eq_st using u_in_XY,
+    
+    rw [←dim_u_k, dim, u_eq_st, simplex_disjoint_card],
+    have st_dim : ↑(s.card + t.card) - 1 = dim s + dim t + 1, by {simp, linarith, },
+    rw [st_dim],
+    
+    have s_le_dim : dim s ≤ dim_of_complex X, from
+    begin
+      apply finset.le_max',
+      simp only [finset.mem_image, set.mem_to_finset],
+      use s, split, assumption,
+      refl,
+    end,
+    
+    have t_le_dim : dim t ≤ dim_of_complex Y, from
+    begin
+      apply finset.le_max',
+      simp only [finset.mem_image, set.mem_to_finset],
+      use t, split, assumption,
+      refl,
+    end,
+    
+    linarith, },
+
+  { have n_dim : n ∈ finset.image dim X.simplices.to_finset, by apply finset.max'_mem,
+    have m_dim : m ∈ finset.image dim Y.simplices.to_finset, by apply finset.max'_mem,
+    simp only [finset.mem_image, set.mem_to_finset] at n_dim m_dim,
+    
+    choose s s_in_X dim_s_n using n_dim,
+    choose t t_in_Y dim_t_m using m_dim,
+    have st_dim : ↑(s.card + t.card) - 1 = dim s + dim t + 1, by {simp, linarith, },
+    simp only [←dim_s_n, ←dim_t_m, ←st_dim, ←simplex_disjoint_card],
+    
+    apply finset.le_max',
+    simp only [finset.mem_image, set.mem_to_finset],
+    use (s ⊔ₛ t), split,
+    
+    rw [simplicial_join_mem],
+    use s, split, assumption,
+    use t, split, assumption,
+    refl,
+    
+    unfold dim, },
 end
 
 -- Show that, for disjoint complexes, projection to the first coordinate is a coercion.
@@ -2096,7 +3780,85 @@ end
 lemma join_fst_proj_is_coe
     (X Y : simplicial_complex α)
   : disjoint (vertices X) (vertices Y) → set.inj_on (prod.fst) (vertices (X ⋆ Y))
-:= sorry
+:= begin
+  intro X_disj_Y,
+  simp only [set.inj_on, vertices_set_of, simplicial_join, set.mem_set_of],
+  simp only [vertices_set_of, set.disjoint_iff_forall_ne, set.mem_set_of] at X_disj_Y,
+
+  intros x₁ x₁_in_lhs x₂ x₂_in_rhs,
+
+  choose s₁ s₁_in_join x₁_in_s₁ using x₁_in_lhs,
+  choose u₁ u₁_in_X v₁ v₁_in_Y uv₁_eq_s₁ using s₁_in_join,
+  rw [←uv₁_eq_s₁, simplex_disjoint_mem] at x₁_in_s₁,
+
+  choose s₂ s₂_in_join x₂_in_s₂ using x₂_in_rhs,
+  choose u₂ u₂_in_X v₂ v₂_in_Y uv₂_eq_s₂ using s₂_in_join,
+  rw [←uv₂_eq_s₂, simplex_disjoint_mem] at x₂_in_s₂,
+
+  cases x₁_in_s₁ with x₁_in_X x₁_in_Y;
+  cases x₂_in_s₂ with x₂_in_X x₂_in_Y,
+
+  -- x₁, x₂ ∈ X case.
+  intros x₁_eq_x₂,
+
+  choose x₁_in_u₁ x₁_zero using x₁_in_X,
+  choose x₂_in_u₂ x₂_zero using x₂_in_X,
+  rw [←x₂_zero] at x₁_zero,
+  rw [prod.ext_iff],
+  split; assumption,
+
+  -- x₁ ∈ X, x₂ ∈ Y case.
+  contrapose,
+  intros x₁_neq_x₂,
+
+  choose x₁_in_u₁ x₁_zero using x₁_in_X,
+  choose x₂_in_v₂ x₂_one using x₂_in_Y,
+
+  have H₁ : ∃ (s : finset α) (H : s ∈ X.simplices), x₁.fst ∈ s, from
+  begin
+    use u₁, split; assumption,
+  end, 
+  specialize X_disj_Y x₁.fst H₁,
+
+  have H₂ : ∃ (s : finset α) (H : s ∈ Y.simplices), x₂.fst ∈ s, from
+  begin
+    use v₂, split; assumption,
+  end,
+  specialize X_disj_Y x₂.fst H₂,
+
+  assumption,
+
+  -- x₁ ∈ Y, x₂ ∈ X case.
+  contrapose,
+  intros x₁_neq_x₂,
+
+  choose x₁_in_v₁ x₁_one using x₁_in_Y,
+  choose x₂_in_u₂ x₂_zero using x₂_in_X,
+
+  have H₂ : ∃ (s : finset α) (H : s ∈ X.simplices), x₂.fst ∈ s, from
+  begin
+    use u₂, split; assumption,
+  end,
+  specialize X_disj_Y x₂.fst H₂,
+
+  have H₁ : ∃ (s : finset α) (H : s ∈ Y.simplices), x₁.fst ∈ s, from
+  begin
+    use v₁, split; assumption,
+  end, 
+  specialize X_disj_Y x₁.fst H₁,
+
+  rw [←ne.def, ne_comm],
+  assumption,
+
+  -- x₁, x₂ ∈ Y case.
+  intros x₁_eq_x₂,
+
+  choose x₁_in_v₁ x₁_one using x₁_in_Y,
+  choose x₂_in_v₂ x₂_one using x₂_in_Y,
+  rw [←x₂_one] at x₁_one,
+  rw [prod.ext_iff],
+  split; assumption,
+end
 
 def join_fst
     {X Y : simplicial_complex α}
@@ -2110,7 +3872,136 @@ lemma join_proj_vertices_mem
     (x : α)
     (H : disjoint (vertices X) (vertices Y))
   : x ∈ vertices ((π₁ H)[(X ⋆ Y)]) ↔ x ∈ vertices X ∨ x ∈ vertices Y
-:= sorry
+:= begin
+  simp only [vertices_set_of, simplicial_image, simplicial_join, set.mem_set_of, join_fst],
+  split,
+
+  -- x ∈ X ⋆ Y case.
+  intros x_in_join,
+  choose u u_in_img x_in_u using x_in_join,
+  choose v v_in_join proj_v_u using u_in_img,
+  choose s s_in_X t t_in_Y st_eq_v using v_in_join,
+
+  rw [←proj_v_u, finset.mem_image] at x_in_u,
+  choose y y_in_v proj_y_x using x_in_u,
+  rw [←st_eq_v, simplex_disjoint_mem] at y_in_v,
+  cases y_in_v with y_in_X y_in_Y,
+
+  left,
+  choose y_in_s y_zero using y_in_X,
+  subst proj_y_x,
+  use s, split; assumption,
+
+  right,
+  choose y_in_t y_one using y_in_Y,
+  subst proj_y_x,
+  use t, split; assumption,
+
+  -- x ∈ X ∪ Y case.
+  intros x_in_union,
+  cases x_in_union with x_in_X x_in_Y,
+
+  -- x ∈ X subcase.
+  choose s s_in_X x_in_s using x_in_X,
+  use s, split,
+  use (s ⊔ₛ ∅), split,
+
+  use s, split, assumption,
+  use ∅, split, apply simplicial_complex_empty_simplex,
+  refl,
+
+  simp only [simplex_disjoint_union, finset.image_union, finset.empty_product, finset.image_empty, finset.union_empty],
+  simp only [finset.ext_iff, finset.mem_image],
+  intros a,
+  split,
+
+  intros a_in_img,
+  choose b b_in_prod proj_b_a using a_in_img,
+  simp only [finset.mem_product] at b_in_prod,
+  choose b_in_s b_zero using b_in_prod,
+  subst proj_b_a,
+  assumption,
+
+  intros a_in_s,
+  use (a, 0), split,
+  simp only [finset.mem_product, prod.fst, prod.snd, finset.mem_singleton],
+  split, assumption, refl,
+  simp only [prod.fst],
+  assumption,
+
+  -- x ∈ Y subcase.
+  choose t t_in_Y x_in_t using x_in_Y,
+  use t, split,
+  use (∅ ⊔ₛ t), split,
+
+  use ∅, split, apply simplicial_complex_empty_simplex,
+  use t, split, assumption,
+  refl,
+
+  simp only [simplex_disjoint_union, finset.image_union, finset.empty_product, finset.image_empty, finset.empty_union],
+  simp only [finset.ext_iff, finset.mem_image],
+  intros a,
+  split,
+
+  intros a_in_img,
+  choose b b_in_prod proj_b_a using a_in_img,
+  simp only [finset.mem_product] at b_in_prod,
+  choose b_in_s b_one using b_in_prod,
+  subst proj_b_a,
+  assumption,
+
+  intros a_in_s,
+  use (a, 1), split,
+  simp only [finset.mem_product, prod.fst, prod.snd, finset.mem_singleton],
+  split, assumption, refl,
+  simp only [prod.fst],
+  assumption,
+end
+
+lemma simplex_disjoint_union_prod_fst
+    (s t : finset α)
+  : finset.image prod.fst (s ⊔ₛ t) = s ∪ t
+:= begin
+  simp only [simplex_disjoint_union, finset.image_union, finset.ext_iff, finset.mem_image, finset.mem_union],
+  intro x,
+  split,
+
+  intro x_in_img,
+  cases x_in_img with x_in_s x_in_t,
+
+  left,
+  choose y y_in_prod proj_y_x using x_in_s,
+  simp only [finset.mem_product] at y_in_prod,
+  choose y_in_s y_zero using y_in_prod,
+  subst proj_y_x,
+  assumption,
+
+  right,
+  choose y y_in_prod proj_y_x using x_in_t,
+  simp only [finset.mem_product] at y_in_prod,
+  choose y_in_t y_one using y_in_prod,
+  subst proj_y_x,
+  assumption,
+
+  intro x_in_st,
+  cases x_in_st with x_in_s x_in_t,
+
+  left,
+  use (x, 0), split,
+  simp only [finset.mem_product],
+  split,
+  assumption,
+  apply finset.mem_singleton_self,
+  simp only [prod.fst],
+
+  right,
+  use (x, 1), split,
+  simp only [finset.mem_product],
+  split,
+  assumption,
+  apply finset.mem_singleton_self,
+  simp only [prod.fst],
+end
 
 lemma join_proj_mem
     (X Y : simplicial_complex α)
@@ -2118,7 +4009,32 @@ lemma join_proj_mem
     (H : disjoint (vertices X) (vertices Y))
   : s ∈ ((π₁ H)[(X ⋆ Y)]).simplices ↔ ∃ (t ∈ X.simplices) (u ∈ Y.simplices), s = t ∪ u
 := begin
-  sorry
+  simp only [simplicial_image, simplicial_join, join_fst, set.mem_set_of],
+  split,
+
+  -- s ∈ X ⋆ Y case.
+  intros s_in_join,
+  choose v v_in_join proj_v_s using s_in_join,
+  choose t t_in_X u u_in_Y tu_eq_v using v_in_join,
+
+  rw [←tu_eq_v, simplex_disjoint_union_prod_fst] at proj_v_s,
+  use t, split, assumption,
+  use u, split, assumption,
+  symmetry,
+  assumption,
+
+  -- s X ∪ Y case.
+  intro x_decomp,
+  choose t t_in_X u u_in_Y s_eq_tu using x_decomp,
+  rw [←simplex_disjoint_union_prod_fst] at s_eq_tu,
+
+  use (t ⊔ₛ u), split,
+  use t, split, assumption,
+  use u, split, assumption,
+  refl,
+
+  symmetry,
+  assumption,
 end
 
 lemma join_proj_disj_union_mem
@@ -2129,7 +4045,56 @@ lemma join_proj_disj_union_mem
       ∃ (s₁ t₁ ∈ X.simplices) (s₂ t₂ ∈ Y.simplices),
         s = s₁ ∪ s₂ ∧ t = t₁ ∪ t₂ ∧ (s₁ ∪ t₁ ∈ X.simplices) ∧ (s₂ ∪ t₂ ∈ Y.simplices)
 := begin
-  sorry
+  rw [join_proj_mem],
+  split,
+
+  -- s ∪ t ∈ X ⋆ Y case.
+  intro st_in_join,
+  choose u u_in_X v v_in_X st_eq_uv using st_in_join,
+
+  use (s ∩ u), split,
+  apply X.subset_closed u,
+  assumption,
+  apply finset.inter_subset_right,
+
+  use (t ∩ u), split,
+  apply X.subset_closed u,
+  assumption,
+  apply finset.inter_subset_right,
+
+  use (s ∩ v), split,
+  apply Y.subset_closed v,
+  assumption,
+  apply finset.inter_subset_right,
+
+  use (t ∩ v), split,
+  apply Y.subset_closed v,
+  assumption,
+  apply finset.inter_subset_right,
+
+  split,
+  rw [←finset.inter_distrib_left, ←st_eq_uv, finset.union_comm, finset.inter_union_self],
+  
+  split,
+  rw [←finset.inter_distrib_left, ←st_eq_uv, finset.inter_union_self],
+
+  split,
+  rw [←finset.inter_distrib_right, st_eq_uv, finset.inter_comm, finset.union_comm, finset.inter_union_self],
+  assumption,
+
+  rw [←finset.inter_distrib_right, st_eq_uv, finset.inter_comm, finset.inter_union_self],
+  assumption,
+
+  -- s ∪ t decomp case.
+  intro st_decomp,
+  choose s₁ s₁_in_X t₁ t₁_in_X s₂ s₂_in_Y t₂ t₂_in_Y st_decomp using st_decomp,
+  choose s_decomp t_decomp st₁_in_X st₂_in_Y using st_decomp,
+
+  use (s₁ ∪ t₁), split, assumption,
+  use (s₂ ∪ t₂), split, assumption,
+
+  rw [finset.union_comm s₂, finset.union_assoc, ←finset.union_assoc t₁, finset.union_comm (t₁ ∪ t₂), ←finset.union_assoc],
+  rw [←s_decomp, ←t_decomp],
 end
 
 -- General result on existence of coercion for complexes over ℕ
@@ -2137,10 +4102,38 @@ end
 def finite_nat_complex_bound
     (X : simplicial_complex ℕ) [fintype X.simplices]
   : ℕ
-:= match (vertices X).to_finset.max with
-   | some n := n
-   | none   := 0
-   end
+:= ((vertices X) ∪ {(0 : ℕ)}).to_finset.max'
+    (begin
+      rw [set.to_finset_nonempty, set.union_nonempty],
+      right,
+      apply set.singleton_nonempty,
+    end)
+
+lemma finite_nat_complex_bound_ne
+    (X : simplicial_complex ℕ) [fintype X.simplices]
+    [X_ne : (vertices X).to_finset.nonempty]
+  : finite_nat_complex_bound X = (vertices X).to_finset.max' X_ne
+:= begin
+  simp only [finite_nat_complex_bound, le_antisymm_iff],
+  split,
+
+  rw [finset.max'_le_iff],
+  intros y y_in_X,
+  rw [set.mem_to_finset, set.mem_union, set.mem_singleton_iff, ←set.mem_to_finset] at y_in_X,
+  cases y_in_X with y_in_X y_zero,
+
+  apply finset.le_max',
+  assumption,
+
+  rw [y_zero],
+  apply zero_le,
+
+  rw [finset.max'_le_iff],
+  intros y y_in_X,
+  apply finset.le_max',
+  rw [set.mem_to_finset, set.mem_union, set.mem_singleton_iff, ←set.mem_to_finset],
+  left, assumption,
+end
 
 def join_nat_proj_map
     (X Y : simplicial_complex ℕ) [fintype X.simplices]
@@ -2150,7 +4143,134 @@ def join_nat_proj_map
 lemma join_nat_proj_is_coe
     (X Y : simplicial_complex ℕ) [fintype X.simplices]
   : set.inj_on (join_nat_proj_map X Y) (vertices (X ⋆ Y))
-:= sorry
+:= begin
+  simp only [set.inj_on, simplicial_join_mem_vertices, join_nat_proj_map],
+  simp only [set.mem_set_of, simplicial_join_mem, ite_eq_iff],
+  intros x₁ x₁_in_join x₂ x₂_in_join x₁_eq_x₂,
+
+  cases x₁_in_join with x₁_in_X x₁_in_Y;
+  cases x₂_in_join with x₂_in_X x₂_in_Y,
+
+  -- x₁, x₂ ∈ X case.
+  choose x₁_in_X x₁_zero using x₁_in_X,
+  choose x₂_in_X x₂_zero using x₂_in_X,
+
+  cases x₁_eq_x₂ with x₁_eq_x₂ contra,
+  choose x₁_zero x₁_eq_x₂ using x₁_eq_x₂,
+  rw [@comm _ eq, ite_eq_iff] at x₁_eq_x₂,
+
+  cases x₁_eq_x₂ with x₁_eq_x₂ contra,
+  choose x₂_zero x₁_eq_x₂ using x₁_eq_x₂,
+  rw [prod.ext_iff],
+  split,
+  symmetry,
+  assumption,
+  rw [←x₂_zero] at x₁_zero,
+  assumption,
+
+  choose contra H using contra,
+  contradiction,
+
+  choose contra H using contra,
+  contradiction,
+
+  -- x₁ ∈ X, x₂ ∈ Y case.
+  choose x₁_in_X x₁_zero using x₁_in_X,
+  choose x₂_in_Y x₂_one using x₂_in_Y,
+
+  cases x₁_eq_x₂ with x₁_eq_x₂ contra,
+  choose x₁_zero x₁_eq_x₂ using x₁_eq_x₂,
+  rw [@comm _ eq, ite_eq_iff] at x₁_eq_x₂,
+
+  cases x₁_eq_x₂ with contra x₁_eq_x₂,
+  choose contra H using contra,
+  have x₂_nonzero : x₂.snd ≠ 0, by omega,
+  contradiction,
+
+  choose x₂_nonzero x₁_eq_x₂ using x₁_eq_x₂,
+  have x₁_le_bound : x₁.fst ≤ finite_nat_complex_bound X, from
+  begin
+    by_cases X_ne : vertices X = ∅,
+    rw [X_ne] at x₁_in_X,
+    have contra : x₁.fst ∉ ∅, from
+    begin
+      apply set.not_mem_empty,
+    end,
+    contradiction,
+
+    rw [←ne.def, ←set.nonempty_iff_ne_empty, ←set.to_finset_nonempty] at X_ne,
+    rw [@finite_nat_complex_bound_ne X _ X_ne],
+
+    apply finset.le_max',
+    rw [set.mem_to_finset],
+    assumption,
+  end,
+
+  have x₁_lt_x₂_bound : x₁.fst < x₂.fst + finite_nat_complex_bound X + 1, by omega,
+  have contra : x₂.fst + finite_nat_complex_bound X + 1 ≠ x₁.fst, by exact ne_of_gt x₁_lt_x₂_bound,
+  contradiction,
+
+  choose contra H using contra,
+  contradiction,
+
+  -- x₁ ∈ Y, x₂ ∈ X case.
+  choose x₁_in_Y x₁_one using x₁_in_Y,
+  choose x₂_in_X x₂_zero using x₂_in_X,
+
+  cases x₁_eq_x₂ with contra x₁_eq_x₂,
+  choose contra H using contra,
+  have x₁_nonzero : x₁.snd ≠ 0, by omega,
+  contradiction,
+
+  choose x₁_zero x₁_eq_x₂ using x₁_eq_x₂,
+  rw [@comm _ eq, ite_eq_iff] at x₁_eq_x₂,
+  cases x₁_eq_x₂ with x₁_eq_x₂ contra,
+
+  choose x₂_nonzero x₁_eq_x₂ using x₁_eq_x₂,
+  have x₂_le_bound : x₂.fst ≤ finite_nat_complex_bound X, from
+  begin
+    simp only [finite_nat_complex_bound],
+    apply finset.le_max',
+    rw [set.mem_to_finset, set.mem_union],
+    left, assumption,
+  end,
+
+  have x₂_lt_x₁_bound : x₂.fst < x₁.fst + finite_nat_complex_bound X + 1, by omega,
+  have contra : x₂.fst ≠ x₁.fst + finite_nat_complex_bound X + 1, by exact ne_of_lt x₂_lt_x₁_bound,
+  contradiction,
+
+  choose contra H using contra,
+  have x₂_nonzero : x₂.snd ≠ 0, by omega,
+  contradiction,
+
+  -- x₁, x₂ ∈ Y case.
+  choose x₁_in_Y x₁_one using x₁_in_Y,
+  choose x₂_in_Y x₂_one using x₂_in_Y,
+
+  cases x₁_eq_x₂ with contra x₁_eq_x₂,
+  choose contra H using contra,
+  have x₁_nonzero : x₁.snd ≠ 0, by omega,
+  contradiction,
+
+  choose x₁_nonzero x₁_eq_x₂ using x₁_eq_x₂,
+  rw [@comm _ eq, ite_eq_iff] at x₁_eq_x₂,
+  cases x₁_eq_x₂ with contra x₁_eq_x₂,
+
+  choose contra H using contra,
+  have x₂_nonzero : x₂.snd ≠ 0, by omega,
+  contradiction,
+
+  choose x₂_nonzero x₁_eq_x₂ using x₁_eq_x₂,
+  have x₁_fst_eq_x₂_fst : x₁.fst = x₂.fst, from
+  begin
+    rw [nat.add_assoc, nat.add_assoc] at x₁_eq_x₂,
+    symmetry,
+    apply nat.add_right_cancel x₁_eq_x₂,
+  end,
+  rw [←x₂_one] at x₁_one,
+  rw [prod.ext_iff],
+  split; assumption,
+end
 
 def join_nat_proj
     (X Y : simplicial_complex ℕ) [fintype X.simplices]
